Removed Explicit RefNode semantics
Replaced the explicit semantics for RefNode with sequential node
semantics and fixed everything that broke.

Graph/IRNodeHierarchy.thy
@@ -229,6 +229,7 @@ fun is_sequential_node :: "IRNode \<Rightarrow> bool" where
   "is_sequential_node (LoopBeginNode _ _ _ _) = True" |
   "is_sequential_node (LoopExitNode _ _ _) = True" |
   "is_sequential_node (MergeNode _ _ _) = True" |
+  "is_sequential_node (RefNode _) = True" |
   "is_sequential_node _ = False"
 
 text \<open>
