Tests/ConditionalEliminationTests.thy
@@ -4,6 +4,7 @@ theory ConditionalEliminationTests
 imports
   Optimizations.ConditionalElimination
   Graph.Comparison
+  Tests.IRGraphSort
 begin
 
 text \<open>
@@ -21,129 +22,910 @@ phase on the unoptimized graph and assert that the optimized graph expected by G
 to that which our Isabelle phase generates.
 \<close>
 
+definition ConditionalEliminationPhaseAnalysisStart where
+  "ConditionalEliminationPhaseAnalysisStart = ([], [])"
 
-(* initial: ConditionalEliminationTest1_test1Snippet_basic*)
-definition ConditionalEliminationTest1_test1Snippet_basic_initial :: IRGraph where
-  "ConditionalEliminationTest1_test1Snippet_basic_initial = irgraph [
-  (0, (StartNode  (Some 2) 7), VoidStamp),
+(* initial: ConditionalEliminationTest13_testSnippet12*)
+definition ConditionalEliminationTest13_testSnippet12_initial :: IRGraph where  "ConditionalEliminationTest13_testSnippet12_initial = irgraph [
+  (0, (StartNode (Some 2) 13), VoidStamp),
   (1, (ParameterNode 0), IntegerStamp 32 (-2147483648) (2147483647)),
-  (2, (FrameState []  None None None), IllegalStamp),
+  (2, (FrameState [] None None None), IllegalStamp),
+  (3, (ConstantNode (IntVal 32 (-1))), IntegerStamp 32 (-1) (-1)),
+  (4, (FrameState [] None None None), IllegalStamp),
+  (5, (ConstantNode (IntVal 32 (-2147483648))), IntegerStamp 32 (-2147483648) (-2147483648)),
+  (6, (AddNode 1 5), IntegerStamp 32 (-2147483648) (2147483647)),
+  (7, (ConstantNode (IntVal 32 (2147483647))), IntegerStamp 32 (2147483647) (2147483647)),
+  (8, (FrameState [] None None None), IllegalStamp),
+  (9, (FrameState [] (Some 8) None None), IllegalStamp),
+  (10, (IntegerEqualsNode 6 7), VoidStamp),
+  (11, (BeginNode 18), VoidStamp),
+  (12, (BeginNode 20), VoidStamp),
+  (13, (IfNode 10 12 11), VoidStamp),
+  (14, (IntegerEqualsNode 1 3), VoidStamp),
+  (15, (ConstantNode (IntVal 32 (0))), IntegerStamp 32 (0) (0)),
+  (16, (ConstantNode (IntVal 32 (1))), IntegerStamp 32 (1) (1)),
+  (17, (ConditionalNode 14 15 16), IntegerStamp 32 (0) (1)),
+  (18, (EndNode), VoidStamp),
+  (19, (MergeNode  [18, 20] (Some 23) 27), VoidStamp),
+  (20, (EndNode), VoidStamp),
+  (21, (ValuePhiNode 21  [3, 17] 19), IntegerStamp 32 (-1) (1)),
+  (22, (FrameState [] (Some 8) None None), IllegalStamp),
+  (23, (FrameState [] (Some 22) None None), IllegalStamp),
+  (24, (IntegerEqualsNode 21 3), VoidStamp),
+  (25, (BeginNode 33), VoidStamp),
+  (26, (BeginNode 28), VoidStamp),
+  (27, (IfNode 24 26 25), VoidStamp),
+  (28, (EndNode), VoidStamp),
+  (29, (MergeNode  [28, 30] (Some 36) 37), VoidStamp),
+  (30, (EndNode), VoidStamp),
+  (31, (BeginNode 34), VoidStamp),
+  (32, (BeginNode 30), VoidStamp),
+  (33, (IfNode 14 31 32), VoidStamp),
+  (34, (StoreFieldNode 34 ''org.graalvm.compiler.core.test.ConditionalEliminationTestBase::sink1'' 15 (Some 35) None 39), VoidStamp),
+  (35, (FrameState [] None None None), IllegalStamp),
+  (36, (FrameState [] None None None), IllegalStamp),
+  (37, (StoreFieldNode 37 ''org.graalvm.compiler.core.test.ConditionalEliminationTestBase::sink0'' 3 (Some 38) None 41), VoidStamp),
+  (38, (FrameState [] None None None), IllegalStamp),
+  (39, (EndNode), VoidStamp),
+  (40, (MergeNode  [39, 41] (Some 42) 43), VoidStamp),
+  (41, (EndNode), VoidStamp),
+  (42, (FrameState [] None None None), IllegalStamp),
+  (43, (ReturnNode None None), VoidStamp)
+  ]"
+
+(* final: ConditionalEliminationTest13_testSnippet12*)
+definition ConditionalEliminationTest13_testSnippet12_final :: IRGraph where  "ConditionalEliminationTest13_testSnippet12_final = irgraph [
+  (0, (StartNode (Some 2) 13), VoidStamp),
+  (1, (ParameterNode 0), IntegerStamp 32 (-2147483648) (2147483647)),
+  (2, (FrameState [] None None None), IllegalStamp),
+  (3, (ConstantNode (IntVal 32 (-1))), IntegerStamp 32 (-1) (-1)),
+  (4, (FrameState [] None None None), IllegalStamp),
+  (5, (ConstantNode (IntVal 32 (-2147483648))), IntegerStamp 32 (-2147483648) (-2147483648)),
+  (6, (AddNode 1 5), IntegerStamp 32 (-2147483648) (2147483647)),
+  (7, (ConstantNode (IntVal 32 (2147483647))), IntegerStamp 32 (2147483647) (2147483647)),
+  (8, (FrameState [] None None None), IllegalStamp),
+  (9, (FrameState [] (Some 8) None None), IllegalStamp),
+  (10, (IntegerEqualsNode 6 7), VoidStamp),
+  (11, (BeginNode 18), VoidStamp),
+  (12, (BeginNode 20), VoidStamp),
+  (13, (IfNode 10 12 11), VoidStamp),
+  (14, (IntegerEqualsNode 1 3), VoidStamp),
+  (15, (ConstantNode (IntVal 32 (0))), IntegerStamp 32 (0) (0)),
+  (16, (ConstantNode (IntVal 32 (1))), IntegerStamp 32 (1) (1)),
+  (17, (ConditionalNode 14 15 16), IntegerStamp 32 (0) (1)),
+  (18, (EndNode), VoidStamp),
+  (19, (MergeNode  [18, 20] (Some 23) 27), VoidStamp),
+  (20, (EndNode), VoidStamp),
+  (21, (ValuePhiNode 21  [3, 17] 19), IntegerStamp 32 (-1) (1)),
+  (22, (FrameState [] (Some 8) None None), IllegalStamp),
+  (23, (FrameState [] (Some 22) None None), IllegalStamp),
+  (24, (IntegerEqualsNode 21 3), VoidStamp),
+  (25, (BeginNode 33), VoidStamp),
+  (26, (BeginNode 28), VoidStamp),
+  (27, (IfNode 24 26 25), VoidStamp),
+  (28, (EndNode), VoidStamp),
+  (29, (MergeNode  [28, 30] (Some 36) 37), VoidStamp),
+  (30, (EndNode), VoidStamp),
+  (31, (BeginNode 34), VoidStamp),
+  (32, (BeginNode 30), VoidStamp),
+  (33, (IfNode 14 31 32), VoidStamp),
+  (34, (StoreFieldNode 34 ''org.graalvm.compiler.core.test.ConditionalEliminationTestBase::sink1'' 15 (Some 35) None 39), VoidStamp),
+  (35, (FrameState [] None None None), IllegalStamp),
+  (36, (FrameState [] None None None), IllegalStamp),
+  (37, (StoreFieldNode 37 ''org.graalvm.compiler.core.test.ConditionalEliminationTestBase::sink0'' 3 (Some 38) None 41), VoidStamp),
+  (38, (FrameState [] None None None), IllegalStamp),
+  (39, (EndNode), VoidStamp),
+  (40, (MergeNode  [39, 41] (Some 42) 43), VoidStamp),
+  (41, (EndNode), VoidStamp),
+  (42, (FrameState [] None None None), IllegalStamp),
+  (43, (ReturnNode None None), VoidStamp)
+  ]"
+
+value "
+  eqGraph
+  (Predicate.the
+    (ConditionalEliminationPhase_i_i_o
+      ConditionalEliminationTest13_testSnippet12_initial
+      (0, {}, ConditionalEliminationPhaseAnalysisStart)
+    ))
+  ConditionalEliminationTest13_testSnippet12_final
+"
+
+value "
+  diffNodesGraph
+  (Predicate.the
+    (ConditionalEliminationPhase_i_i_o
+      ConditionalEliminationTest13_testSnippet12_initial
+      (0, {}, ConditionalEliminationPhaseAnalysisStart)
+    ))
+  ConditionalEliminationTest13_testSnippet12_final
+"
+
+value "
+  diffNodesInfo
+  (Predicate.the
+    (ConditionalEliminationPhase_i_i_o
+      ConditionalEliminationTest13_testSnippet12_initial
+      (0, {}, ConditionalEliminationPhaseAnalysisStart)
+    ))
+  ConditionalEliminationTest13_testSnippet12_final
+"
+
+
+(* initial: ConditionalEliminationTest13_testSnippet13*)
+definition ConditionalEliminationTest13_testSnippet13_initial :: IRGraph where  "ConditionalEliminationTest13_testSnippet13_initial = irgraph [
+  (0, (StartNode (Some 2) 6), VoidStamp),
+  (1, (ParameterNode 0), IntegerStamp 32 (-2147483648) (2147483647)),
+  (2, (FrameState [] None None None), IllegalStamp),
   (3, (ConstantNode (IntVal 32 (0))), IntegerStamp 32 (0) (0)),
-  (4, (IntegerEqualsNode 1 3), VoidStamp),
+  (4, (ConstantNode (IntVal 32 (1))), IntegerStamp 32 (1) (1)),
+  (5, (FrameState [] None None None), IllegalStamp),
+  (6, (LoadFieldNode 6 ''org.graalvm.compiler.core.test.ConditionalEliminationTestBase::sink0'' None 7), IntegerStamp 32 (-2147483648) (2147483647)),
+  (7, (LoadFieldNode 7 ''org.graalvm.compiler.core.test.ConditionalEliminationTestBase::sink1'' None 9), IntegerStamp 32 (-2147483648) (2147483647)),
+  (8, (AddNode 6 7), IntegerStamp 32 (-2147483648) (2147483647)),
+  (9, (LoadFieldNode 9 ''org.graalvm.compiler.core.test.ConditionalEliminationTestBase::sink2'' None 14), IntegerStamp 32 (-2147483648) (2147483647)),
+  (10, (AddNode 8 9), IntegerStamp 32 (-2147483648) (2147483647)),
+  (11, (IntegerEqualsNode 10 3), VoidStamp),
+  (12, (BeginNode 17), VoidStamp),
+  (13, (BeginNode 15), VoidStamp),
+  (14, (IfNode 11 13 12), VoidStamp),
+  (15, (EndNode), VoidStamp),
+  (16, (MergeNode  [15, 17] (Some 20) 25), VoidStamp),
+  (17, (EndNode), VoidStamp),
+  (18, (ValuePhiNode 18  [3, 4] 16), IntegerStamp 32 (0) (1)),
+  (19, (FrameState [] None None None), IllegalStamp),
+  (20, (FrameState [] (Some 19) None None), IllegalStamp),
+  (21, (AddNode 1 18), IntegerStamp 32 (-2147483648) (2147483647)),
+  (22, (IntegerLessThanNode 21 1), VoidStamp),
+  (23, (BeginNode 30), VoidStamp),
+  (24, (BeginNode 41), VoidStamp),
+  (25, (IfNode 22 24 23), VoidStamp),
+  (26, (ConstantNode (IntVal 32 (2147483647))), IntegerStamp 32 (2147483647) (2147483647)),
+  (27, (IntegerEqualsNode 1 26), VoidStamp),
+  (28, (BeginNode 34), VoidStamp),
+  (29, (BeginNode 32), VoidStamp),
+  (30, (IfNode 27 29 28), VoidStamp),
+  (31, (ConstantNode (IntVal 32 (-2))), IntegerStamp 32 (-2) (-2)),
+  (32, (StoreFieldNode 32 ''org.graalvm.compiler.core.test.ConditionalEliminationTestBase::sink2'' 31 (Some 33) None 36), VoidStamp),
+  (33, (FrameState [] None None None), IllegalStamp),
+  (34, (EndNode), VoidStamp),
+  (35, (MergeNode  [34, 36] (Some 37) 38), VoidStamp),
+  (36, (EndNode), VoidStamp),
+  (37, (FrameState [] None None None), IllegalStamp),
+  (38, (StoreFieldNode 38 ''org.graalvm.compiler.core.test.ConditionalEliminationTestBase::sink1'' 3 (Some 39) None 43), VoidStamp),
+  (39, (FrameState [] None None None), IllegalStamp),
+  (40, (ConstantNode (IntVal 32 (-1))), IntegerStamp 32 (-1) (-1)),
+  (41, (StoreFieldNode 41 ''org.graalvm.compiler.core.test.ConditionalEliminationTestBase::sink0'' 40 (Some 42) None 45), VoidStamp),
+  (42, (FrameState [] None None None), IllegalStamp),
+  (43, (EndNode), VoidStamp),
+  (44, (MergeNode  [43, 45] (Some 46) 47), VoidStamp),
+  (45, (EndNode), VoidStamp),
+  (46, (FrameState [] None None None), IllegalStamp),
+  (47, (ReturnNode None None), VoidStamp)
+  ]"
+
+(* final: ConditionalEliminationTest13_testSnippet13*)
+definition ConditionalEliminationTest13_testSnippet13_final :: IRGraph where  "ConditionalEliminationTest13_testSnippet13_final = irgraph [
+  (0, (StartNode (Some 2) 6), VoidStamp),
+  (1, (ParameterNode 0), IntegerStamp 32 (-2147483648) (2147483647)),
+  (2, (FrameState [] None None None), IllegalStamp),
+  (3, (ConstantNode (IntVal 32 (0))), IntegerStamp 32 (0) (0)),
+  (4, (ConstantNode (IntVal 32 (1))), IntegerStamp 32 (1) (1)),
+  (5, (FrameState [] None None None), IllegalStamp),
+  (6, (LoadFieldNode 6 ''org.graalvm.compiler.core.test.ConditionalEliminationTestBase::sink0'' None 7), IntegerStamp 32 (-2147483648) (2147483647)),
+  (7, (LoadFieldNode 7 ''org.graalvm.compiler.core.test.ConditionalEliminationTestBase::sink1'' None 9), IntegerStamp 32 (-2147483648) (2147483647)),
+  (8, (AddNode 6 7), IntegerStamp 32 (-2147483648) (2147483647)),
+  (9, (LoadFieldNode 9 ''org.graalvm.compiler.core.test.ConditionalEliminationTestBase::sink2'' None 14), IntegerStamp 32 (-2147483648) (2147483647)),
+  (10, (AddNode 8 9), IntegerStamp 32 (-2147483648) (2147483647)),
+  (11, (IntegerEqualsNode 10 3), VoidStamp),
+  (12, (BeginNode 17), VoidStamp),
+  (13, (BeginNode 15), VoidStamp),
+  (14, (IfNode 11 13 12), VoidStamp),
+  (15, (EndNode), VoidStamp),
+  (16, (MergeNode  [15, 17] (Some 20) 25), VoidStamp),
+  (17, (EndNode), VoidStamp),
+  (18, (ValuePhiNode 18  [3, 4] 16), IntegerStamp 32 (0) (1)),
+  (19, (FrameState [] None None None), IllegalStamp),
+  (20, (FrameState [] (Some 19) None None), IllegalStamp),
+  (21, (AddNode 1 18), IntegerStamp 32 (-2147483648) (2147483647)),
+  (22, (IntegerLessThanNode 21 1), VoidStamp),
+  (23, (BeginNode 30), VoidStamp),
+  (24, (BeginNode 41), VoidStamp),
+  (25, (IfNode 22 24 23), VoidStamp),
+  (26, (ConstantNode (IntVal 32 (2147483647))), IntegerStamp 32 (2147483647) (2147483647)),
+  (27, (IntegerEqualsNode 1 26), VoidStamp),
+  (28, (BeginNode 34), VoidStamp),
+  (29, (BeginNode 32), VoidStamp),
+  (30, (IfNode 27 29 28), VoidStamp),
+  (31, (ConstantNode (IntVal 32 (-2))), IntegerStamp 32 (-2) (-2)),
+  (32, (StoreFieldNode 32 ''org.graalvm.compiler.core.test.ConditionalEliminationTestBase::sink2'' 31 (Some 33) None 36), VoidStamp),
+  (33, (FrameState [] None None None), IllegalStamp),
+  (34, (EndNode), VoidStamp),
+  (35, (MergeNode  [34, 36] (Some 37) 38), VoidStamp),
+  (36, (EndNode), VoidStamp),
+  (37, (FrameState [] None None None), IllegalStamp),
+  (38, (StoreFieldNode 38 ''org.graalvm.compiler.core.test.ConditionalEliminationTestBase::sink1'' 3 (Some 39) None 43), VoidStamp),
+  (39, (FrameState [] None None None), IllegalStamp),
+  (40, (ConstantNode (IntVal 32 (-1))), IntegerStamp 32 (-1) (-1)),
+  (41, (StoreFieldNode 41 ''org.graalvm.compiler.core.test.ConditionalEliminationTestBase::sink0'' 40 (Some 42) None 45), VoidStamp),
+  (42, (FrameState [] None None None), IllegalStamp),
+  (43, (EndNode), VoidStamp),
+  (44, (MergeNode  [43, 45] (Some 46) 47), VoidStamp),
+  (45, (EndNode), VoidStamp),
+  (46, (FrameState [] None None None), IllegalStamp),
+  (47, (ReturnNode None None), VoidStamp)
+  ]"
+
+values "{g'. (ConditionalEliminationPhase
+      ConditionalEliminationTest13_testSnippet13_initial
+      (0, {}, ConditionalEliminationPhaseAnalysisStart) g')}"
+
+value "
+  eqGraph
+  (Predicate.the
+    (ConditionalEliminationPhase_i_i_o
+      ConditionalEliminationTest13_testSnippet13_initial
+      (0, {}, ConditionalEliminationPhaseAnalysisStart)
+    ))
+  ConditionalEliminationTest13_testSnippet13_final
+"
+
+value "
+  diffNodesGraph
+  (Predicate.the
+    (ConditionalEliminationPhase_i_i_o
+      ConditionalEliminationTest13_testSnippet13_initial
+      (0, {}, ConditionalEliminationPhaseAnalysisStart)
+    ))
+  ConditionalEliminationTest13_testSnippet13_final
+"
+
+value "
+  diffNodesInfo
+  (Predicate.the
+    (ConditionalEliminationPhase_i_i_o
+      ConditionalEliminationTest13_testSnippet13_initial
+      (0, {}, ConditionalEliminationPhaseAnalysisStart)
+    ))
+  ConditionalEliminationTest13_testSnippet13_final
+"
+
+
+(* initial: ConditionalEliminationTest13_testSnippet14*)
+definition ConditionalEliminationTest13_testSnippet14_initial :: IRGraph where  "ConditionalEliminationTest13_testSnippet14_initial = irgraph [
+  (0, (StartNode (Some 2) 6), VoidStamp),
+  (1, (ParameterNode 0), IntegerStamp 32 (-2147483648) (2147483647)),
+  (2, (FrameState [] None None None), IllegalStamp),
+  (3, (ConstantNode (IntVal 32 (0))), IntegerStamp 32 (0) (0)),
+  (4, (ConstantNode (IntVal 32 (1))), IntegerStamp 32 (1) (1)),
+  (5, (FrameState [] None None None), IllegalStamp),
+  (6, (LoadFieldNode 6 ''org.graalvm.compiler.core.test.ConditionalEliminationTestBase::sink0'' None 7), IntegerStamp 32 (-2147483648) (2147483647)),
+  (7, (LoadFieldNode 7 ''org.graalvm.compiler.core.test.ConditionalEliminationTestBase::sink1'' None 9), IntegerStamp 32 (-2147483648) (2147483647)),
+  (8, (AddNode 6 7), IntegerStamp 32 (-2147483648) (2147483647)),
+  (9, (LoadFieldNode 9 ''org.graalvm.compiler.core.test.ConditionalEliminationTestBase::sink2'' None 14), IntegerStamp 32 (-2147483648) (2147483647)),
+  (10, (AddNode 8 9), IntegerStamp 32 (-2147483648) (2147483647)),
+  (11, (IntegerEqualsNode 10 3), VoidStamp),
+  (12, (BeginNode 17), VoidStamp),
+  (13, (BeginNode 15), VoidStamp),
+  (14, (IfNode 11 13 12), VoidStamp),
+  (15, (EndNode), VoidStamp),
+  (16, (MergeNode  [15, 17] (Some 20) 25), VoidStamp),
+  (17, (EndNode), VoidStamp),
+  (18, (ValuePhiNode 18  [3, 4] 16), IntegerStamp 32 (0) (1)),
+  (19, (FrameState [] None None None), IllegalStamp),
+  (20, (FrameState [] (Some 19) None None), IllegalStamp),
+  (21, (AddNode 1 18), IntegerStamp 32 (-2147483648) (2147483647)),
+  (22, (IntegerLessThanNode 1 21), VoidStamp),
+  (23, (BeginNode 41), VoidStamp),
+  (24, (BeginNode 30), VoidStamp),
+  (25, (IfNode 22 24 23), VoidStamp),
+  (26, (ConstantNode (IntVal 32 (2147483647))), IntegerStamp 32 (2147483647) (2147483647)),
+  (27, (IntegerEqualsNode 1 26), VoidStamp),
+  (28, (BeginNode 34), VoidStamp),
+  (29, (BeginNode 32), VoidStamp),
+  (30, (IfNode 27 29 28), VoidStamp),
+  (31, (ConstantNode (IntVal 32 (-2))), IntegerStamp 32 (-2) (-2)),
+  (32, (StoreFieldNode 32 ''org.graalvm.compiler.core.test.ConditionalEliminationTestBase::sink2'' 31 (Some 33) None 36), VoidStamp),
+  (33, (FrameState [] None None None), IllegalStamp),
+  (34, (EndNode), VoidStamp),
+  (35, (MergeNode  [34, 36] (Some 37) 38), VoidStamp),
+  (36, (EndNode), VoidStamp),
+  (37, (FrameState [] None None None), IllegalStamp),
+  (38, (StoreFieldNode 38 ''org.graalvm.compiler.core.test.ConditionalEliminationTestBase::sink1'' 3 (Some 39) None 43), VoidStamp),
+  (39, (FrameState [] None None None), IllegalStamp),
+  (40, (ConstantNode (IntVal 32 (-1))), IntegerStamp 32 (-1) (-1)),
+  (41, (StoreFieldNode 41 ''org.graalvm.compiler.core.test.ConditionalEliminationTestBase::sink0'' 40 (Some 42) None 45), VoidStamp),
+  (42, (FrameState [] None None None), IllegalStamp),
+  (43, (EndNode), VoidStamp),
+  (44, (MergeNode  [43, 45] (Some 46) 47), VoidStamp),
+  (45, (EndNode), VoidStamp),
+  (46, (FrameState [] None None None), IllegalStamp),
+  (47, (ReturnNode None None), VoidStamp)
+  ]"
+
+(* final: ConditionalEliminationTest13_testSnippet14*)
+definition ConditionalEliminationTest13_testSnippet14_final :: IRGraph where  "ConditionalEliminationTest13_testSnippet14_final = irgraph [
+  (0, (StartNode (Some 2) 6), VoidStamp),
+  (1, (ParameterNode 0), IntegerStamp 32 (-2147483648) (2147483647)),
+  (2, (FrameState [] None None None), IllegalStamp),
+  (3, (ConstantNode (IntVal 32 (0))), IntegerStamp 32 (0) (0)),
+  (4, (ConstantNode (IntVal 32 (1))), IntegerStamp 32 (1) (1)),
+  (5, (FrameState [] None None None), IllegalStamp),
+  (6, (LoadFieldNode 6 ''org.graalvm.compiler.core.test.ConditionalEliminationTestBase::sink0'' None 7), IntegerStamp 32 (-2147483648) (2147483647)),
+  (7, (LoadFieldNode 7 ''org.graalvm.compiler.core.test.ConditionalEliminationTestBase::sink1'' None 9), IntegerStamp 32 (-2147483648) (2147483647)),
+  (8, (AddNode 6 7), IntegerStamp 32 (-2147483648) (2147483647)),
+  (9, (LoadFieldNode 9 ''org.graalvm.compiler.core.test.ConditionalEliminationTestBase::sink2'' None 14), IntegerStamp 32 (-2147483648) (2147483647)),
+  (10, (AddNode 8 9), IntegerStamp 32 (-2147483648) (2147483647)),
+  (11, (IntegerEqualsNode 10 3), VoidStamp),
+  (12, (BeginNode 17), VoidStamp),
+  (13, (BeginNode 15), VoidStamp),
+  (14, (IfNode 11 13 12), VoidStamp),
+  (15, (EndNode), VoidStamp),
+  (16, (MergeNode  [15, 17] (Some 20) 25), VoidStamp),
+  (17, (EndNode), VoidStamp),
+  (18, (ValuePhiNode 18  [3, 4] 16), IntegerStamp 32 (0) (1)),
+  (19, (FrameState [] None None None), IllegalStamp),
+  (20, (FrameState [] (Some 19) None None), IllegalStamp),
+  (21, (AddNode 1 18), IntegerStamp 32 (-2147483648) (2147483647)),
+  (22, (IntegerLessThanNode 1 21), VoidStamp),
+  (23, (BeginNode 41), VoidStamp),
+  (24, (BeginNode 30), VoidStamp),
+  (25, (IfNode 22 24 23), VoidStamp),
+  (26, (ConstantNode (IntVal 32 (2147483647))), IntegerStamp 32 (2147483647) (2147483647)),
+  (27, (IntegerEqualsNode 1 26), VoidStamp),
+  (28, (BeginNode 34), VoidStamp),
+  (29, (BeginNode 32), VoidStamp),
+  (30, (IfNode 48 29 28), VoidStamp),
+  (31, (ConstantNode (IntVal 32 (-2))), IntegerStamp 32 (-2) (-2)),
+  (32, (StoreFieldNode 32 ''org.graalvm.compiler.core.test.ConditionalEliminationTestBase::sink2'' 31 (Some 33) None 36), VoidStamp),
+  (33, (FrameState [] None None None), IllegalStamp),
+  (34, (EndNode), VoidStamp),
+  (35, (MergeNode  [34, 36] (Some 37) 38), VoidStamp),
+  (36, (EndNode), VoidStamp),
+  (37, (FrameState [] None None None), IllegalStamp),
+  (38, (StoreFieldNode 38 ''org.graalvm.compiler.core.test.ConditionalEliminationTestBase::sink1'' 3 (Some 39) None 43), VoidStamp),
+  (39, (FrameState [] None None None), IllegalStamp),
+  (40, (ConstantNode (IntVal 32 (-1))), IntegerStamp 32 (-1) (-1)),
+  (41, (StoreFieldNode 41 ''org.graalvm.compiler.core.test.ConditionalEliminationTestBase::sink0'' 40 (Some 42) None 45), VoidStamp),
+  (42, (FrameState [] None None None), IllegalStamp),
+  (43, (EndNode), VoidStamp),
+  (44, (MergeNode  [43, 45] (Some 46) 47), VoidStamp),
+  (45, (EndNode), VoidStamp),
+  (46, (FrameState [] None None None), IllegalStamp),
+  (47, (ReturnNode None None), VoidStamp),
+  (48, (ConstantNode (IntVal 1 (0))), VoidStamp)
+  ]"
+
+value "
+  eqGraph
+  (Predicate.the
+    (ConditionalEliminationPhase_i_i_o
+      ConditionalEliminationTest13_testSnippet14_initial
+      (0, {}, ConditionalEliminationPhaseAnalysisStart)
+    ))
+  ConditionalEliminationTest13_testSnippet14_final
+"
+
+value "
+  diffNodesGraph
+  (Predicate.the
+    (ConditionalEliminationPhase_i_i_o
+      ConditionalEliminationTest13_testSnippet14_initial
+      (0, {}, ConditionalEliminationPhaseAnalysisStart)
+    ))
+  ConditionalEliminationTest13_testSnippet14_final
+"
+
+value "
+  diffNodesInfo
+  (Predicate.the
+    (ConditionalEliminationPhase_i_i_o
+      ConditionalEliminationTest13_testSnippet14_initial
+      (0, {}, ConditionalEliminationPhaseAnalysisStart)
+    ))
+  ConditionalEliminationTest13_testSnippet14_final
+"
+
+
+(* initial: ConditionalEliminationTest13_testSnippet2*)
+definition ConditionalEliminationTest13_testSnippet2_initial :: IRGraph where  "ConditionalEliminationTest13_testSnippet2_initial = irgraph [
+  (0, (StartNode (Some 2) 8), VoidStamp),
+  (1, (ParameterNode 0), IntegerStamp 32 (-2147483648) (2147483647)),
+  (2, (FrameState [] None None None), IllegalStamp),
+  (3, (ConstantNode (IntVal 32 (0))), IntegerStamp 32 (0) (0)),
+  (4, (ConstantNode (IntVal 32 (1))), IntegerStamp 32 (1) (1)),
+  (5, (IntegerLessThanNode 1 4), VoidStamp),
+  (6, (BeginNode 13), VoidStamp),
+  (7, (BeginNode 23), VoidStamp),
+  (8, (IfNode 5 7 6), VoidStamp),
+  (9, (ConstantNode (IntVal 32 (-1))), IntegerStamp 32 (-1) (-1)),
+  (10, (IntegerEqualsNode 1 9), VoidStamp),
+  (11, (BeginNode 17), VoidStamp),
+  (12, (BeginNode 15), VoidStamp),
+  (13, (IfNode 10 12 11), VoidStamp),
+  (14, (ConstantNode (IntVal 32 (-2))), IntegerStamp 32 (-2) (-2)),
+  (15, (StoreFieldNode 15 ''org.graalvm.compiler.core.test.ConditionalEliminationTestBase::sink2'' 14 (Some 16) None 19), VoidStamp),
+  (16, (FrameState [] None None None), IllegalStamp),
+  (17, (EndNode), VoidStamp),
+  (18, (MergeNode  [17, 19] (Some 20) 21), VoidStamp),
+  (19, (EndNode), VoidStamp),
+  (20, (FrameState [] None None None), IllegalStamp),
+  (21, (StoreFieldNode 21 ''org.graalvm.compiler.core.test.ConditionalEliminationTestBase::sink1'' 3 (Some 22) None 25), VoidStamp),
+  (22, (FrameState [] None None None), IllegalStamp),
+  (23, (EndNode), VoidStamp),
+  (24, (MergeNode  [23, 25] (Some 26) 27), VoidStamp),
+  (25, (EndNode), VoidStamp),
+  (26, (FrameState [] None None None), IllegalStamp),
+  (27, (StoreFieldNode 27 ''org.graalvm.compiler.core.test.ConditionalEliminationTestBase::sink0'' 9 (Some 28) None 29), VoidStamp),
+  (28, (FrameState [] None None None), IllegalStamp),
+  (29, (ReturnNode None None), VoidStamp)
+  ]"
+
+(* final: ConditionalEliminationTest13_testSnippet2*)
+definition ConditionalEliminationTest13_testSnippet2_final :: IRGraph where  "ConditionalEliminationTest13_testSnippet2_final = irgraph [
+  (0, (StartNode (Some 2) 8), VoidStamp),
+  (1, (ParameterNode 0), IntegerStamp 32 (-2147483648) (2147483647)),
+  (2, (FrameState [] None None None), IllegalStamp),
+  (3, (ConstantNode (IntVal 32 (0))), IntegerStamp 32 (0) (0)),
+  (4, (ConstantNode (IntVal 32 (1))), IntegerStamp 32 (1) (1)),
+  (5, (IntegerLessThanNode 1 4), VoidStamp),
+  (6, (BeginNode 13), VoidStamp),
+  (7, (BeginNode 23), VoidStamp),
+  (8, (IfNode 5 7 6), VoidStamp),
+  (9, (ConstantNode (IntVal 32 (-1))), IntegerStamp 32 (-1) (-1)),
+  (10, (IntegerEqualsNode 1 9), VoidStamp),
+  (11, (BeginNode 17), VoidStamp),
+  (12, (BeginNode 15), VoidStamp),
+  (13, (IfNode 30 12 11), VoidStamp),
+  (14, (ConstantNode (IntVal 32 (-2))), IntegerStamp 32 (-2) (-2)),
+  (15, (StoreFieldNode 15 ''org.graalvm.compiler.core.test.ConditionalEliminationTestBase::sink2'' 14 (Some 16) None 19), VoidStamp),
+  (16, (FrameState [] None None None), IllegalStamp),
+  (17, (EndNode), VoidStamp),
+  (18, (MergeNode  [17, 19] (Some 20) 21), VoidStamp),
+  (19, (EndNode), VoidStamp),
+  (20, (FrameState [] None None None), IllegalStamp),
+  (21, (StoreFieldNode 21 ''org.graalvm.compiler.core.test.ConditionalEliminationTestBase::sink1'' 3 (Some 22) None 25), VoidStamp),
+  (22, (FrameState [] None None None), IllegalStamp),
+  (23, (EndNode), VoidStamp),
+  (24, (MergeNode  [23, 25] (Some 26) 27), VoidStamp),
+  (25, (EndNode), VoidStamp),
+  (26, (FrameState [] None None None), IllegalStamp),
+  (27, (StoreFieldNode 27 ''org.graalvm.compiler.core.test.ConditionalEliminationTestBase::sink0'' 9 (Some 28) None 29), VoidStamp),
+  (28, (FrameState [] None None None), IllegalStamp),
+  (29, (ReturnNode None None), VoidStamp),
+  (30, (ConstantNode (IntVal 1 (0))), VoidStamp)
+  ]"
+
+value "
+  eqGraph
+  (Predicate.the
+    (ConditionalEliminationPhase_i_i_o
+      ConditionalEliminationTest13_testSnippet2_initial
+      (0, {}, ConditionalEliminationPhaseAnalysisStart)
+    ))
+  ConditionalEliminationTest13_testSnippet2_final
+"
+
+value "
+  diffNodesGraph
+  (Predicate.the
+    (ConditionalEliminationPhase_i_i_o
+      ConditionalEliminationTest13_testSnippet2_initial
+      (0, {}, ConditionalEliminationPhaseAnalysisStart)
+    ))
+  ConditionalEliminationTest13_testSnippet2_final
+"
+
+value "
+  diffNodesInfo
+  (Predicate.the
+    (ConditionalEliminationPhase_i_i_o
+      ConditionalEliminationTest13_testSnippet2_initial
+      (0, {}, ConditionalEliminationPhaseAnalysisStart)
+    ))
+  ConditionalEliminationTest13_testSnippet2_final
+"
+
+
+(* initial: ConditionalEliminationTest13_testSnippet3*)
+definition ConditionalEliminationTest13_testSnippet3_initial :: IRGraph where  "ConditionalEliminationTest13_testSnippet3_initial = irgraph [
+  (0, (StartNode (Some 2) 8), VoidStamp),
+  (1, (ParameterNode 0), IntegerStamp 32 (-2147483648) (2147483647)),
+  (2, (FrameState [] None None None), IllegalStamp),
+  (3, (ConstantNode (IntVal 32 (0))), IntegerStamp 32 (0) (0)),
+  (4, (ConstantNode (IntVal 32 (1))), IntegerStamp 32 (1) (1)),
+  (5, (IntegerLessThanNode 1 4), VoidStamp),
+  (6, (BeginNode 12), VoidStamp),
+  (7, (BeginNode 22), VoidStamp),
+  (8, (IfNode 5 7 6), VoidStamp),
+  (9, (IntegerEqualsNode 1 4), VoidStamp),
+  (10, (BeginNode 16), VoidStamp),
+  (11, (BeginNode 14), VoidStamp),
+  (12, (IfNode 9 11 10), VoidStamp),
+  (13, (ConstantNode (IntVal 32 (-2))), IntegerStamp 32 (-2) (-2)),
+  (14, (StoreFieldNode 14 ''org.graalvm.compiler.core.test.ConditionalEliminationTestBase::sink2'' 13 (Some 15) None 18), VoidStamp),
+  (15, (FrameState [] None None None), IllegalStamp),
+  (16, (EndNode), VoidStamp),
+  (17, (MergeNode  [16, 18] (Some 19) 20), VoidStamp),
+  (18, (EndNode), VoidStamp),
+  (19, (FrameState [] None None None), IllegalStamp),
+  (20, (StoreFieldNode 20 ''org.graalvm.compiler.core.test.ConditionalEliminationTestBase::sink1'' 3 (Some 21) None 24), VoidStamp),
+  (21, (FrameState [] None None None), IllegalStamp),
+  (22, (EndNode), VoidStamp),
+  (23, (MergeNode  [22, 24] (Some 25) 27), VoidStamp),
+  (24, (EndNode), VoidStamp),
+  (25, (FrameState [] None None None), IllegalStamp),
+  (26, (ConstantNode (IntVal 32 (-1))), IntegerStamp 32 (-1) (-1)),
+  (27, (StoreFieldNode 27 ''org.graalvm.compiler.core.test.ConditionalEliminationTestBase::sink0'' 26 (Some 28) None 29), VoidStamp),
+  (28, (FrameState [] None None None), IllegalStamp),
+  (29, (ReturnNode None None), VoidStamp)
+  ]"
+
+(* final: ConditionalEliminationTest13_testSnippet3*)
+definition ConditionalEliminationTest13_testSnippet3_final :: IRGraph where  "ConditionalEliminationTest13_testSnippet3_final = irgraph [
+  (0, (StartNode (Some 2) 8), VoidStamp),
+  (1, (ParameterNode 0), IntegerStamp 32 (-2147483648) (2147483647)),
+  (2, (FrameState [] None None None), IllegalStamp),
+  (3, (ConstantNode (IntVal 32 (0))), IntegerStamp 32 (0) (0)),
+  (4, (ConstantNode (IntVal 32 (1))), IntegerStamp 32 (1) (1)),
+  (5, (IntegerLessThanNode 1 4), VoidStamp),
+  (6, (BeginNode 12), VoidStamp),
+  (7, (BeginNode 22), VoidStamp),
+  (8, (IfNode 5 7 6), VoidStamp),
+  (9, (IntegerEqualsNode 1 4), VoidStamp),
+  (10, (BeginNode 16), VoidStamp),
+  (11, (BeginNode 14), VoidStamp),
+  (12, (IfNode 9 11 10), VoidStamp),
+  (13, (ConstantNode (IntVal 32 (-2))), IntegerStamp 32 (-2) (-2)),
+  (14, (StoreFieldNode 14 ''org.graalvm.compiler.core.test.ConditionalEliminationTestBase::sink2'' 13 (Some 15) None 18), VoidStamp),
+  (15, (FrameState [] None None None), IllegalStamp),
+  (16, (EndNode), VoidStamp),
+  (17, (MergeNode  [16, 18] (Some 19) 20), VoidStamp),
+  (18, (EndNode), VoidStamp),
+  (19, (FrameState [] None None None), IllegalStamp),
+  (20, (StoreFieldNode 20 ''org.graalvm.compiler.core.test.ConditionalEliminationTestBase::sink1'' 3 (Some 21) None 24), VoidStamp),
+  (21, (FrameState [] None None None), IllegalStamp),
+  (22, (EndNode), VoidStamp),
+  (23, (MergeNode  [22, 24] (Some 25) 27), VoidStamp),
+  (24, (EndNode), VoidStamp),
+  (25, (FrameState [] None None None), IllegalStamp),
+  (26, (ConstantNode (IntVal 32 (-1))), IntegerStamp 32 (-1) (-1)),
+  (27, (StoreFieldNode 27 ''org.graalvm.compiler.core.test.ConditionalEliminationTestBase::sink0'' 26 (Some 28) None 29), VoidStamp),
+  (28, (FrameState [] None None None), IllegalStamp),
+  (29, (ReturnNode None None), VoidStamp)
+  ]"
+
+value "
+  eqGraph
+  (Predicate.the
+    (ConditionalEliminationPhase_i_i_o
+      ConditionalEliminationTest13_testSnippet3_initial
+      (0, {}, ConditionalEliminationPhaseAnalysisStart)
+    ))
+  ConditionalEliminationTest13_testSnippet3_final
+"
+
+value "
+  diffNodesGraph
+  (Predicate.the
+    (ConditionalEliminationPhase_i_i_o
+      ConditionalEliminationTest13_testSnippet3_initial
+      (0, {}, ConditionalEliminationPhaseAnalysisStart)
+    ))
+  ConditionalEliminationTest13_testSnippet3_final
+"
+
+value "
+  diffNodesInfo
+  (Predicate.the
+    (ConditionalEliminationPhase_i_i_o
+      ConditionalEliminationTest13_testSnippet3_initial
+      (0, {}, ConditionalEliminationPhaseAnalysisStart)
+    ))
+  ConditionalEliminationTest13_testSnippet3_final
+"
+
+
+(* initial: ConditionalEliminationTest13_testSnippet5*)
+definition ConditionalEliminationTest13_testSnippet5_initial :: IRGraph where  "ConditionalEliminationTest13_testSnippet5_initial = irgraph [
+  (0, (StartNode (Some 2) 7), VoidStamp),
+  (1, (ParameterNode 0), IntegerStamp 32 (-2147483648) (2147483647)),
+  (2, (FrameState [] None None None), IllegalStamp),
+  (3, (ConstantNode (IntVal 32 (0))), IntegerStamp 32 (0) (0)),
+  (4, (IntegerLessThanNode 1 3), VoidStamp),
   (5, (BeginNode 22), VoidStamp),
+  (6, (BeginNode 12), VoidStamp),
+  (7, (IfNode 4 6 5), VoidStamp),
+  (8, (ConstantNode (IntVal 32 (-1))), IntegerStamp 32 (-1) (-1)),
+  (9, (IntegerEqualsNode 1 8), VoidStamp),
+  (10, (BeginNode 16), VoidStamp),
+  (11, (BeginNode 14), VoidStamp),
+  (12, (IfNode 9 11 10), VoidStamp),
+  (13, (ConstantNode (IntVal 32 (-2))), IntegerStamp 32 (-2) (-2)),
+  (14, (StoreFieldNode 14 ''org.graalvm.compiler.core.test.ConditionalEliminationTestBase::sink2'' 13 (Some 15) None 18), VoidStamp),
+  (15, (FrameState [] None None None), IllegalStamp),
+  (16, (EndNode), VoidStamp),
+  (17, (MergeNode  [16, 18] (Some 19) 20), VoidStamp),
+  (18, (EndNode), VoidStamp),
+  (19, (FrameState [] None None None), IllegalStamp),
+  (20, (StoreFieldNode 20 ''org.graalvm.compiler.core.test.ConditionalEliminationTestBase::sink1'' 3 (Some 21) None 24), VoidStamp),
+  (21, (FrameState [] None None None), IllegalStamp),
+  (22, (EndNode), VoidStamp),
+  (23, (MergeNode  [22, 24] (Some 25) 26), VoidStamp),
+  (24, (EndNode), VoidStamp),
+  (25, (FrameState [] None None None), IllegalStamp),
+  (26, (StoreFieldNode 26 ''org.graalvm.compiler.core.test.ConditionalEliminationTestBase::sink0'' 8 (Some 27) None 28), VoidStamp),
+  (27, (FrameState [] None None None), IllegalStamp),
+  (28, (ReturnNode None None), VoidStamp)
+  ]"
+
+(* final: ConditionalEliminationTest13_testSnippet5*)
+definition ConditionalEliminationTest13_testSnippet5_final :: IRGraph where  "ConditionalEliminationTest13_testSnippet5_final = irgraph [
+  (0, (StartNode (Some 2) 7), VoidStamp),
+  (1, (ParameterNode 0), IntegerStamp 32 (-2147483648) (2147483647)),
+  (2, (FrameState [] None None None), IllegalStamp),
+  (3, (ConstantNode (IntVal 32 (0))), IntegerStamp 32 (0) (0)),
+  (4, (IntegerLessThanNode 1 3), VoidStamp),
+  (5, (BeginNode 22), VoidStamp),
+  (6, (BeginNode 12), VoidStamp),
+  (7, (IfNode 4 6 5), VoidStamp),
+  (8, (ConstantNode (IntVal 32 (-1))), IntegerStamp 32 (-1) (-1)),
+  (9, (IntegerEqualsNode 1 8), VoidStamp),
+  (10, (BeginNode 16), VoidStamp),
+  (11, (BeginNode 14), VoidStamp),
+  (12, (IfNode 9 11 10), VoidStamp),
+  (13, (ConstantNode (IntVal 32 (-2))), IntegerStamp 32 (-2) (-2)),
+  (14, (StoreFieldNode 14 ''org.graalvm.compiler.core.test.ConditionalEliminationTestBase::sink2'' 13 (Some 15) None 18), VoidStamp),
+  (15, (FrameState [] None None None), IllegalStamp),
+  (16, (EndNode), VoidStamp),
+  (17, (MergeNode  [16, 18] (Some 19) 20), VoidStamp),
+  (18, (EndNode), VoidStamp),
+  (19, (FrameState [] None None None), IllegalStamp),
+  (20, (StoreFieldNode 20 ''org.graalvm.compiler.core.test.ConditionalEliminationTestBase::sink1'' 3 (Some 21) None 24), VoidStamp),
+  (21, (FrameState [] None None None), IllegalStamp),
+  (22, (EndNode), VoidStamp),
+  (23, (MergeNode  [22, 24] (Some 25) 26), VoidStamp),
+  (24, (EndNode), VoidStamp),
+  (25, (FrameState [] None None None), IllegalStamp),
+  (26, (StoreFieldNode 26 ''org.graalvm.compiler.core.test.ConditionalEliminationTestBase::sink0'' 8 (Some 27) None 28), VoidStamp),
+  (27, (FrameState [] None None None), IllegalStamp),
+  (28, (ReturnNode None None), VoidStamp)
+  ]"
+
+value "
+  eqGraph
+  (Predicate.the
+    (ConditionalEliminationPhase_i_i_o
+      ConditionalEliminationTest13_testSnippet5_initial
+      (0, {}, ConditionalEliminationPhaseAnalysisStart)
+    ))
+  ConditionalEliminationTest13_testSnippet5_final
+"
+
+value "
+  diffNodesGraph
+  (Predicate.the
+    (ConditionalEliminationPhase_i_i_o
+      ConditionalEliminationTest13_testSnippet5_initial
+      (0, {}, ConditionalEliminationPhaseAnalysisStart)
+    ))
+  ConditionalEliminationTest13_testSnippet5_final
+"
+
+value "
+  diffNodesInfo
+  (Predicate.the
+    (ConditionalEliminationPhase_i_i_o
+      ConditionalEliminationTest13_testSnippet5_initial
+      (0, {}, ConditionalEliminationPhaseAnalysisStart)
+    ))
+  ConditionalEliminationTest13_testSnippet5_final
+"
+
+
+(* initial: ConditionalEliminationTest13_testSnippet6*)
+definition ConditionalEliminationTest13_testSnippet6_initial :: IRGraph where  "ConditionalEliminationTest13_testSnippet6_initial = irgraph [
+  (0, (StartNode (Some 2) 7), VoidStamp),
+  (1, (ParameterNode 0), IntegerStamp 32 (-2147483648) (2147483647)),
+  (2, (FrameState [] None None None), IllegalStamp),
+  (3, (ConstantNode (IntVal 32 (0))), IntegerStamp 32 (0) (0)),
+  (4, (IntegerLessThanNode 1 3), VoidStamp),
+  (5, (BeginNode 21), VoidStamp),
   (6, (BeginNode 11), VoidStamp),
   (7, (IfNode 4 6 5), VoidStamp),
-  (8, (IntegerLessThanNode 1 3), VoidStamp),
+  (8, (IntegerEqualsNode 1 3), VoidStamp),
   (9, (BeginNode 15), VoidStamp),
   (10, (BeginNode 13), VoidStamp),
   (11, (IfNode 8 10 9), VoidStamp),
-  (12, (ConstantNode (IntVal 32 (200))), IntegerStamp 32 (200) (200)),
-  (13, (StoreFieldNode 13 ''org.graalvm.compiler.core.test.ConditionalEliminationTest1::sink3'' 12  (Some 14)  None 17), VoidStamp),
-  (14, (FrameState []  None None None), IllegalStamp),
+  (12, (ConstantNode (IntVal 32 (-2))), IntegerStamp 32 (-2) (-2)),
+  (13, (StoreFieldNode 13 ''org.graalvm.compiler.core.test.ConditionalEliminationTestBase::sink2'' 12 (Some 14) None 17), VoidStamp),
+  (14, (FrameState [] None None None), IllegalStamp),
   (15, (EndNode), VoidStamp),
-  (16, (MergeNode  [15, 17]  (Some 18) 20), VoidStamp),
+  (16, (MergeNode  [15, 17] (Some 18) 19), VoidStamp),
   (17, (EndNode), VoidStamp),
-  (18, (FrameState []  None None None), IllegalStamp),
-  (19, (ConstantNode (IntVal 32 (1))), IntegerStamp 32 (1) (1)),
-  (20, (StoreFieldNode 20 ''org.graalvm.compiler.core.test.ConditionalEliminationTestBase::sink1'' 19  (Some 21)  None 24), VoidStamp),
-  (21, (FrameState []  None None None), IllegalStamp),
-  (22, (EndNode), VoidStamp),
-  (23, (MergeNode  [22, 24]  (Some 25) 26), VoidStamp),
-  (24, (EndNode), VoidStamp),
-  (25, (FrameState []  None None None), IllegalStamp),
-  (26, (StoreFieldNode 26 ''org.graalvm.compiler.core.test.ConditionalEliminationTestBase::sink0'' 3  (Some 27)  None 28), VoidStamp),
-  (27, (FrameState []  None None None), IllegalStamp),
-  (28, (ReturnNode  None  None), VoidStamp)
+  (18, (FrameState [] None None None), IllegalStamp),
+  (19, (StoreFieldNode 19 ''org.graalvm.compiler.core.test.ConditionalEliminationTestBase::sink1'' 3 (Some 20) None 23), VoidStamp),
+  (20, (FrameState [] None None None), IllegalStamp),
+  (21, (EndNode), VoidStamp),
+  (22, (MergeNode  [21, 23] (Some 24) 26), VoidStamp),
+  (23, (EndNode), VoidStamp),
+  (24, (FrameState [] None None None), IllegalStamp),
+  (25, (ConstantNode (IntVal 32 (-1))), IntegerStamp 32 (-1) (-1)),
+  (26, (StoreFieldNode 26 ''org.graalvm.compiler.core.test.ConditionalEliminationTestBase::sink0'' 25 (Some 27) None 28), VoidStamp),
+  (27, (FrameState [] None None None), IllegalStamp),
+  (28, (ReturnNode None None), VoidStamp)
   ]"
 
-(* final: ConditionalEliminationTest1_test1Snippet_basic*)
-definition ConditionalEliminationTest1_test1Snippet_basic_final :: IRGraph where
-  "ConditionalEliminationTest1_test1Snippet_basic_final = irgraph [
-  (0, (StartNode  (Some 2) 7), VoidStamp),
+(* final: ConditionalEliminationTest13_testSnippet6*)
+definition ConditionalEliminationTest13_testSnippet6_final :: IRGraph where  "ConditionalEliminationTest13_testSnippet6_final = irgraph [
+  (0, (StartNode (Some 2) 7), VoidStamp),
   (1, (ParameterNode 0), IntegerStamp 32 (-2147483648) (2147483647)),
-  (2, (FrameState []  None None None), IllegalStamp),
+  (2, (FrameState [] None None None), IllegalStamp),
   (3, (ConstantNode (IntVal 32 (0))), IntegerStamp 32 (0) (0)),
-  (4, (IntegerEqualsNode 1 3), VoidStamp),
-  (5, (BeginNode 22), VoidStamp),
+  (4, (IntegerLessThanNode 1 3), VoidStamp),
+  (5, (BeginNode 21), VoidStamp),
   (6, (BeginNode 11), VoidStamp),
   (7, (IfNode 4 6 5), VoidStamp),
-  (8, (IntegerLessThanNode 1 3), VoidStamp),
+  (8, (IntegerEqualsNode 1 3), VoidStamp),
   (9, (BeginNode 15), VoidStamp),
   (10, (BeginNode 13), VoidStamp),
   (11, (IfNode 29 10 9), VoidStamp),
-  (12, (ConstantNode (IntVal 32 (200))), IntegerStamp 32 (200) (200)),
-  (13, (StoreFieldNode 13 ''org.graalvm.compiler.core.test.ConditionalEliminationTest1::sink3'' 12  (Some 14)  None 17), VoidStamp),
-  (14, (FrameState []  None None None), IllegalStamp),
+  (12, (ConstantNode (IntVal 32 (-2))), IntegerStamp 32 (-2) (-2)),
+  (13, (StoreFieldNode 13 ''org.graalvm.compiler.core.test.ConditionalEliminationTestBase::sink2'' 12 (Some 14) None 17), VoidStamp),
+  (14, (FrameState [] None None None), IllegalStamp),
   (15, (EndNode), VoidStamp),
-  (16, (MergeNode  [15, 17]  (Some 18) 20), VoidStamp),
+  (16, (MergeNode  [15, 17] (Some 18) 19), VoidStamp),
   (17, (EndNode), VoidStamp),
-  (18, (FrameState []  None None None), IllegalStamp),
-  (19, (ConstantNode (IntVal 32 (1))), IntegerStamp 32 (1) (1)),
-  (20, (StoreFieldNode 20 ''org.graalvm.compiler.core.test.ConditionalEliminationTestBase::sink1'' 19  (Some 21)  None 24), VoidStamp),
-  (21, (FrameState []  None None None), IllegalStamp),
-  (22, (EndNode), VoidStamp),
-  (23, (MergeNode  [22, 24]  (Some 25) 26), VoidStamp),
-  (24, (EndNode), VoidStamp),
-  (25, (FrameState []  None None None), IllegalStamp),
-  (26, (StoreFieldNode 26 ''org.graalvm.compiler.core.test.ConditionalEliminationTestBase::sink0'' 3  (Some 27)  None 28), VoidStamp),
-  (27, (FrameState []  None None None), IllegalStamp),
-  (28, (ReturnNode  None  None), VoidStamp),
+  (18, (FrameState [] None None None), IllegalStamp),
+  (19, (StoreFieldNode 19 ''org.graalvm.compiler.core.test.ConditionalEliminationTestBase::sink1'' 3 (Some 20) None 23), VoidStamp),
+  (20, (FrameState [] None None None), IllegalStamp),
+  (21, (EndNode), VoidStamp),
+  (22, (MergeNode  [21, 23] (Some 24) 26), VoidStamp),
+  (23, (EndNode), VoidStamp),
+  (24, (FrameState [] None None None), IllegalStamp),
+  (25, (ConstantNode (IntVal 32 (-1))), IntegerStamp 32 (-1) (-1)),
+  (26, (StoreFieldNode 26 ''org.graalvm.compiler.core.test.ConditionalEliminationTestBase::sink0'' 25 (Some 27) None 28), VoidStamp),
+  (27, (FrameState [] None None None), IllegalStamp),
+  (28, (ReturnNode None None), VoidStamp),
   (29, (ConstantNode (IntVal 1 (0))), VoidStamp)
   ]"
 
-values "{g' . ConditionalEliminationPhase ConditionalEliminationTest1_test1Snippet_basic_initial  (0, {}, [], []) g'}"
+value "
+  eqGraph
+  (Predicate.the
+    (ConditionalEliminationPhase_i_i_o
+      ConditionalEliminationTest13_testSnippet6_initial
+      (0, {}, ConditionalEliminationPhaseAnalysisStart)
+    ))
+  ConditionalEliminationTest13_testSnippet6_final
+"
 
-definition ConditionalEliminationTest1_test1Snippet_basic_isabelle :: IRGraph where
-"ConditionalEliminationTest1_test1Snippet_basic_isabelle = irgraph [
-    (11, IfNode 29 10 9, VoidStamp),
-    (29, ConstantNode (IntVal 1 0), IntegerStamp 32 (- 2147483648) 2147483647),
-    (0, StartNode (Some 2) 7, VoidStamp),
-    (1, ParameterNode 0, IntegerStamp 32 (- 2147483648) 2147483647),
-    (2, FrameState [] None None None, IllegalStamp),
-    (3, ConstantNode (IntVal 32 0), IntegerStamp 32 0 0),
-    (4, IntegerEqualsNode 1 3, VoidStamp), (5, BeginNode 22, VoidStamp),
-    (6, BeginNode 11, VoidStamp), (7, IfNode 4 6 5, VoidStamp),
-    (8, IntegerLessThanNode 1 3, VoidStamp), (9, BeginNode 15, VoidStamp),
-    (10, BeginNode 13, VoidStamp), (11, IfNode 8 10 9, VoidStamp),
-    (12, ConstantNode (IntVal 32 200), IntegerStamp 32 200 200),
-    (13,
-     StoreFieldNode 13
-      ''org.graalvm.compiler.core.test.ConditionalEliminationTest1::sink3'' 12
-      (Some 14) None 17,
-     VoidStamp),
-    (14, FrameState [] None None None, IllegalStamp), (15, EndNode, VoidStamp),
-    (16, MergeNode [15, 17] (Some 18) 20, VoidStamp), (17, EndNode, VoidStamp),
-    (18, FrameState [] None None None, IllegalStamp),
-    (19, ConstantNode (IntVal 32 1), IntegerStamp 32 1 1),
-    (20,
-     StoreFieldNode 20
-      ''org.graalvm.compiler.core.test.ConditionalEliminationTestBase::sink1'' 19
-      (Some 21) None 24,
-     VoidStamp),
-    (21, FrameState [] None None None, IllegalStamp), (22, EndNode, VoidStamp),
-    (23, MergeNode [22, 24] (Some 25) 26, VoidStamp), (24, EndNode, VoidStamp),
-    (25, FrameState [] None None None, IllegalStamp),
-    (26,
-     StoreFieldNode 26
-      ''org.graalvm.compiler.core.test.ConditionalEliminationTestBase::sink0'' 3
-      (Some 27) None 28,
-     VoidStamp),
-    (27, FrameState [] None None None, IllegalStamp),
-    (28, ReturnNode None None, VoidStamp)]"
+value "
+  diffNodesGraph
+  (Predicate.the
+    (ConditionalEliminationPhase_i_i_o
+      ConditionalEliminationTest13_testSnippet6_initial
+      (0, {}, ConditionalEliminationPhaseAnalysisStart)
+    ))
+  ConditionalEliminationTest13_testSnippet6_final
+"
 
-(* compare test1Snippet_basic, isabelle optimised graph vs graal optimised graph *)
-value "eqGraph ConditionalEliminationTest1_test1Snippet_basic_isabelle ConditionalEliminationTest1_test1Snippet_basic_final"
+value "
+  diffNodesInfo
+  (Predicate.the
+    (ConditionalEliminationPhase_i_i_o
+      ConditionalEliminationTest13_testSnippet6_initial
+      (0, {}, ConditionalEliminationPhaseAnalysisStart)
+    ))
+  ConditionalEliminationTest13_testSnippet6_final
+"
 
 
+(* initial: ConditionalEliminationTest13_testSnippet7*)
+definition ConditionalEliminationTest13_testSnippet7_initial :: IRGraph where  "ConditionalEliminationTest13_testSnippet7_initial = irgraph [
+  (0, (StartNode (Some 2) 8), VoidStamp),
+  (1, (ParameterNode 0), IntegerStamp 32 (-2147483648) (2147483647)),
+  (2, (FrameState [] None None None), IllegalStamp),
+  (3, (ConstantNode (IntVal 32 (0))), IntegerStamp 32 (0) (0)),
+  (4, (ConstantNode (IntVal 32 (1))), IntegerStamp 32 (1) (1)),
+  (5, (IntegerLessThanNode 1 4), VoidStamp),
+  (6, (BeginNode 12), VoidStamp),
+  (7, (BeginNode 22), VoidStamp),
+  (8, (IfNode 5 7 6), VoidStamp),
+  (9, (IntegerEqualsNode 1 3), VoidStamp),
+  (10, (BeginNode 16), VoidStamp),
+  (11, (BeginNode 14), VoidStamp),
+  (12, (IfNode 9 11 10), VoidStamp),
+  (13, (ConstantNode (IntVal 32 (-2))), IntegerStamp 32 (-2) (-2)),
+  (14, (StoreFieldNode 14 ''org.graalvm.compiler.core.test.ConditionalEliminationTestBase::sink2'' 13 (Some 15) None 18), VoidStamp),
+  (15, (FrameState [] None None None), IllegalStamp),
+  (16, (EndNode), VoidStamp),
+  (17, (MergeNode  [16, 18] (Some 19) 20), VoidStamp),
+  (18, (EndNode), VoidStamp),
+  (19, (FrameState [] None None None), IllegalStamp),
+  (20, (StoreFieldNode 20 ''org.graalvm.compiler.core.test.ConditionalEliminationTestBase::sink1'' 3 (Some 21) None 24), VoidStamp),
+  (21, (FrameState [] None None None), IllegalStamp),
+  (22, (EndNode), VoidStamp),
+  (23, (MergeNode  [22, 24] (Some 25) 27), VoidStamp),
+  (24, (EndNode), VoidStamp),
+  (25, (FrameState [] None None None), IllegalStamp),
+  (26, (ConstantNode (IntVal 32 (-1))), IntegerStamp 32 (-1) (-1)),
+  (27, (StoreFieldNode 27 ''org.graalvm.compiler.core.test.ConditionalEliminationTestBase::sink0'' 26 (Some 28) None 29), VoidStamp),
+  (28, (FrameState [] None None None), IllegalStamp),
+  (29, (ReturnNode None None), VoidStamp)
+  ]"
 
+(* final: ConditionalEliminationTest13_testSnippet7*)
+definition ConditionalEliminationTest13_testSnippet7_final :: IRGraph where  "ConditionalEliminationTest13_testSnippet7_final = irgraph [
+  (0, (StartNode (Some 2) 8), VoidStamp),
+  (1, (ParameterNode 0), IntegerStamp 32 (-2147483648) (2147483647)),
+  (2, (FrameState [] None None None), IllegalStamp),
+  (3, (ConstantNode (IntVal 32 (0))), IntegerStamp 32 (0) (0)),
+  (4, (ConstantNode (IntVal 32 (1))), IntegerStamp 32 (1) (1)),
+  (5, (IntegerLessThanNode 1 4), VoidStamp),
+  (6, (BeginNode 12), VoidStamp),
+  (7, (BeginNode 22), VoidStamp),
+  (8, (IfNode 5 7 6), VoidStamp),
+  (9, (IntegerEqualsNode 1 3), VoidStamp),
+  (10, (BeginNode 16), VoidStamp),
+  (11, (BeginNode 14), VoidStamp),
+  (12, (IfNode 30 11 10), VoidStamp),
+  (13, (ConstantNode (IntVal 32 (-2))), IntegerStamp 32 (-2) (-2)),
+  (14, (StoreFieldNode 14 ''org.graalvm.compiler.core.test.ConditionalEliminationTestBase::sink2'' 13 (Some 15) None 18), VoidStamp),
+  (15, (FrameState [] None None None), IllegalStamp),
+  (16, (EndNode), VoidStamp),
+  (17, (MergeNode  [16, 18] (Some 19) 20), VoidStamp),
+  (18, (EndNode), VoidStamp),
+  (19, (FrameState [] None None None), IllegalStamp),
+  (20, (StoreFieldNode 20 ''org.graalvm.compiler.core.test.ConditionalEliminationTestBase::sink1'' 3 (Some 21) None 24), VoidStamp),
+  (21, (FrameState [] None None None), IllegalStamp),
+  (22, (EndNode), VoidStamp),
+  (23, (MergeNode  [22, 24] (Some 25) 27), VoidStamp),
+  (24, (EndNode), VoidStamp),
+  (25, (FrameState [] None None None), IllegalStamp),
+  (26, (ConstantNode (IntVal 32 (-1))), IntegerStamp 32 (-1) (-1)),
+  (27, (StoreFieldNode 27 ''org.graalvm.compiler.core.test.ConditionalEliminationTestBase::sink0'' 26 (Some 28) None 29), VoidStamp),
+  (28, (FrameState [] None None None), IllegalStamp),
+  (29, (ReturnNode None None), VoidStamp),
+  (30, (ConstantNode (IntVal 1 (0))), VoidStamp)
+  ]"
+
+value "
+  eqGraph
+  (Predicate.the
+    (ConditionalEliminationPhase_i_i_o
+      ConditionalEliminationTest13_testSnippet7_initial
+      (0, {}, ConditionalEliminationPhaseAnalysisStart)
+    ))
+  ConditionalEliminationTest13_testSnippet7_final
+"
+
+value "
+  diffNodesGraph
+  (Predicate.the
+    (ConditionalEliminationPhase_i_i_o
+      ConditionalEliminationTest13_testSnippet7_initial
+      (0, {}, ConditionalEliminationPhaseAnalysisStart)
+    ))
+  ConditionalEliminationTest13_testSnippet7_final
+"
+
+value "
+  diffNodesInfo
+  (Predicate.the
+    (ConditionalEliminationPhase_i_i_o
+      ConditionalEliminationTest13_testSnippet7_initial
+      (0, {}, ConditionalEliminationPhaseAnalysisStart)
+    ))
+  ConditionalEliminationTest13_testSnippet7_final
+"
 
 
 (* initial: ConditionalEliminationTest1_test1Snippet*)
-definition ConditionalEliminationTest1_test1Snippet_initial :: IRGraph where
-  "ConditionalEliminationTest1_test1Snippet_initial = irgraph [
-  (0, (StartNode  (Some 2) 7), VoidStamp),
+definition ConditionalEliminationTest1_test1Snippet_initial :: IRGraph where  "ConditionalEliminationTest1_test1Snippet_initial = irgraph [
+  (0, (StartNode (Some 2) 7), VoidStamp),
   (1, (ParameterNode 0), IntegerStamp 32 (-2147483648) (2147483647)),
-  (2, (FrameState []  None None None), IllegalStamp),
+  (2, (FrameState [] None None None), IllegalStamp),
   (3, (ConstantNode (IntVal 32 (0))), IntegerStamp 32 (0) (0)),
   (4, (IntegerEqualsNode 1 3), VoidStamp),
   (5, (BeginNode 39), VoidStamp),
@@ -155,52 +937,51 @@ definition ConditionalEliminationTest1_test1Snippet_initial :: IRGraph where
   (11, (BeginNode 14), VoidStamp),
   (12, (IfNode 9 11 10), VoidStamp),
   (13, (ConstantNode (IntVal 32 (100))), IntegerStamp 32 (100) (100)),
-  (14, (StoreFieldNode 14 ''org.graalvm.compiler.core.test.ConditionalEliminationTestBase::sink2'' 13  (Some 15)  None 18), VoidStamp),
-  (15, (FrameState []  None None None), IllegalStamp),
+  (14, (StoreFieldNode 14 ''org.graalvm.compiler.core.test.ConditionalEliminationTestBase::sink2'' 13 (Some 15) None 18), VoidStamp),
+  (15, (FrameState [] None None None), IllegalStamp),
   (16, (EndNode), VoidStamp),
-  (17, (MergeNode  [16, 18]  (Some 19) 24), VoidStamp),
+  (17, (MergeNode  [16, 18] (Some 19) 24), VoidStamp),
   (18, (EndNode), VoidStamp),
-  (19, (FrameState []  None None None), IllegalStamp),
+  (19, (FrameState [] None None None), IllegalStamp),
   (20, (ConstantNode (IntVal 32 (101))), IntegerStamp 32 (101) (101)),
   (21, (IntegerLessThanNode 1 20), VoidStamp),
   (22, (BeginNode 30), VoidStamp),
   (23, (BeginNode 25), VoidStamp),
   (24, (IfNode 21 23 22), VoidStamp),
   (25, (EndNode), VoidStamp),
-  (26, (MergeNode  [25, 27, 34]  (Some 35) 43), VoidStamp),
+  (26, (MergeNode  [25, 27, 34] (Some 35) 43), VoidStamp),
   (27, (EndNode), VoidStamp),
   (28, (BeginNode 32), VoidStamp),
   (29, (BeginNode 27), VoidStamp),
   (30, (IfNode 4 28 29), VoidStamp),
   (31, (ConstantNode (IntVal 32 (200))), IntegerStamp 32 (200) (200)),
-  (32, (StoreFieldNode 32 ''org.graalvm.compiler.core.test.ConditionalEliminationTest1::sink3'' 31  (Some 33)  None 34), VoidStamp),
-  (33, (FrameState []  None None None), IllegalStamp),
+  (32, (StoreFieldNode 32 ''org.graalvm.compiler.core.test.ConditionalEliminationTest1::sink3'' 31 (Some 33) None 34), VoidStamp),
+  (33, (FrameState [] None None None), IllegalStamp),
   (34, (EndNode), VoidStamp),
-  (35, (FrameState []  None None None), IllegalStamp),
+  (35, (FrameState [] None None None), IllegalStamp),
   (36, (ConstantNode (IntVal 32 (2))), IntegerStamp 32 (2) (2)),
   (37, (IntegerEqualsNode 1 36), VoidStamp),
   (38, (BeginNode 45), VoidStamp),
   (39, (EndNode), VoidStamp),
-  (40, (MergeNode  [39, 41, 47]  (Some 48) 49), VoidStamp),
+  (40, (MergeNode  [39, 41, 47] (Some 48) 49), VoidStamp),
   (41, (EndNode), VoidStamp),
   (42, (BeginNode 41), VoidStamp),
   (43, (IfNode 37 42 38), VoidStamp),
   (44, (ConstantNode (IntVal 32 (1))), IntegerStamp 32 (1) (1)),
-  (45, (StoreFieldNode 45 ''org.graalvm.compiler.core.test.ConditionalEliminationTestBase::sink1'' 44  (Some 46)  None 47), VoidStamp),
-  (46, (FrameState []  None None None), IllegalStamp),
+  (45, (StoreFieldNode 45 ''org.graalvm.compiler.core.test.ConditionalEliminationTestBase::sink1'' 44 (Some 46) None 47), VoidStamp),
+  (46, (FrameState [] None None None), IllegalStamp),
   (47, (EndNode), VoidStamp),
-  (48, (FrameState []  None None None), IllegalStamp),
-  (49, (StoreFieldNode 49 ''org.graalvm.compiler.core.test.ConditionalEliminationTestBase::sink0'' 3  (Some 50)  None 51), VoidStamp),
-  (50, (FrameState []  None None None), IllegalStamp),
-  (51, (ReturnNode  None  None), VoidStamp)
+  (48, (FrameState [] None None None), IllegalStamp),
+  (49, (StoreFieldNode 49 ''org.graalvm.compiler.core.test.ConditionalEliminationTestBase::sink0'' 3 (Some 50) None 51), VoidStamp),
+  (50, (FrameState [] None None None), IllegalStamp),
+  (51, (ReturnNode None None), VoidStamp)
   ]"
 
 (* final: ConditionalEliminationTest1_test1Snippet*)
-definition ConditionalEliminationTest1_test1Snippet_final :: IRGraph where
-  "ConditionalEliminationTest1_test1Snippet_final = irgraph [
-  (0, (StartNode  (Some 2) 7), VoidStamp),
+definition ConditionalEliminationTest1_test1Snippet_final :: IRGraph where  "ConditionalEliminationTest1_test1Snippet_final = irgraph [
+  (0, (StartNode (Some 2) 7), VoidStamp),
   (1, (ParameterNode 0), IntegerStamp 32 (-2147483648) (2147483647)),
-  (2, (FrameState []  None None None), IllegalStamp),
+  (2, (FrameState [] None None None), IllegalStamp),
   (3, (ConstantNode (IntVal 32 (0))), IntegerStamp 32 (0) (0)),
   (4, (IntegerEqualsNode 1 3), VoidStamp),
   (5, (BeginNode 39), VoidStamp),
@@ -212,128 +993,84 @@ definition ConditionalEliminationTest1_test1Snippet_final :: IRGraph where
   (11, (BeginNode 14), VoidStamp),
   (12, (IfNode 52 11 10), VoidStamp),
   (13, (ConstantNode (IntVal 32 (100))), IntegerStamp 32 (100) (100)),
-  (14, (StoreFieldNode 14 ''org.graalvm.compiler.core.test.ConditionalEliminationTestBase::sink2'' 13  (Some 15)  None 18), VoidStamp),
-  (15, (FrameState []  None None None), IllegalStamp),
+  (14, (StoreFieldNode 14 ''org.graalvm.compiler.core.test.ConditionalEliminationTestBase::sink2'' 13 (Some 15) None 18), VoidStamp),
+  (15, (FrameState [] None None None), IllegalStamp),
   (16, (EndNode), VoidStamp),
-  (17, (MergeNode  [16, 18]  (Some 19) 24), VoidStamp),
+  (17, (MergeNode  [16, 18] (Some 19) 24), VoidStamp),
   (18, (EndNode), VoidStamp),
-  (19, (FrameState []  None None None), IllegalStamp),
+  (19, (FrameState [] None None None), IllegalStamp),
   (20, (ConstantNode (IntVal 32 (101))), IntegerStamp 32 (101) (101)),
   (21, (IntegerLessThanNode 1 20), VoidStamp),
   (22, (BeginNode 30), VoidStamp),
   (23, (BeginNode 25), VoidStamp),
   (24, (IfNode 53 23 22), VoidStamp),
   (25, (EndNode), VoidStamp),
-  (26, (MergeNode  [25, 27, 34]  (Some 35) 43), VoidStamp),
+  (26, (MergeNode  [25, 27, 34] (Some 35) 43), VoidStamp),
   (27, (EndNode), VoidStamp),
   (28, (BeginNode 32), VoidStamp),
   (29, (BeginNode 27), VoidStamp),
   (30, (IfNode 53 28 29), VoidStamp),
   (31, (ConstantNode (IntVal 32 (200))), IntegerStamp 32 (200) (200)),
-  (32, (StoreFieldNode 32 ''org.graalvm.compiler.core.test.ConditionalEliminationTest1::sink3'' 31  (Some 33)  None 34), VoidStamp),
-  (33, (FrameState []  None None None), IllegalStamp),
+  (32, (StoreFieldNode 32 ''org.graalvm.compiler.core.test.ConditionalEliminationTest1::sink3'' 31 (Some 33) None 34), VoidStamp),
+  (33, (FrameState [] None None None), IllegalStamp),
   (34, (EndNode), VoidStamp),
-  (35, (FrameState []  None None None), IllegalStamp),
+  (35, (FrameState [] None None None), IllegalStamp),
   (36, (ConstantNode (IntVal 32 (2))), IntegerStamp 32 (2) (2)),
   (37, (IntegerEqualsNode 1 36), VoidStamp),
   (38, (BeginNode 45), VoidStamp),
   (39, (EndNode), VoidStamp),
-  (40, (MergeNode  [39, 41, 47]  (Some 48) 49), VoidStamp),
+  (40, (MergeNode  [39, 41, 47] (Some 48) 49), VoidStamp),
   (41, (EndNode), VoidStamp),
   (42, (BeginNode 41), VoidStamp),
   (43, (IfNode 52 42 38), VoidStamp),
   (44, (ConstantNode (IntVal 32 (1))), IntegerStamp 32 (1) (1)),
-  (45, (StoreFieldNode 45 ''org.graalvm.compiler.core.test.ConditionalEliminationTestBase::sink1'' 44  (Some 46)  None 47), VoidStamp),
-  (46, (FrameState []  None None None), IllegalStamp),
+  (45, (StoreFieldNode 45 ''org.graalvm.compiler.core.test.ConditionalEliminationTestBase::sink1'' 44 (Some 46) None 47), VoidStamp),
+  (46, (FrameState [] None None None), IllegalStamp),
   (47, (EndNode), VoidStamp),
-  (48, (FrameState []  None None None), IllegalStamp),
-  (49, (StoreFieldNode 49 ''org.graalvm.compiler.core.test.ConditionalEliminationTestBase::sink0'' 3  (Some 50)  None 51), VoidStamp),
-  (50, (FrameState []  None None None), IllegalStamp),
-  (51, (ReturnNode  None  None), VoidStamp),
-  (52, (ConstantNode (IntVal 1 (0))), VoidStamp),
-  (53, (ConstantNode (IntVal 1 (1))), VoidStamp)
+  (48, (FrameState [] None None None), IllegalStamp),
+  (49, (StoreFieldNode 49 ''org.graalvm.compiler.core.test.ConditionalEliminationTestBase::sink0'' 3 (Some 50) None 51), VoidStamp),
+  (50, (FrameState [] None None None), IllegalStamp),
+  (51, (ReturnNode None None), VoidStamp),
+  (52, (LogicConstantNode (IntVal 1 (0))), VoidStamp),
+  (53, (LogicConstantNode (IntVal 1 (1))), VoidStamp)
   ]"
 
-values "{g' . ConditionalEliminationPhase ConditionalEliminationTest1_test1Snippet_initial  (0, {}, [], []) g'}"
-definition ConditionalEliminationTest1_test1Snippet_isabelle :: IRGraph where
-  "ConditionalEliminationTest1_test1Snippet_isabelle = irgraph
-    [(43, IfNode 54 42 38, VoidStamp),
-    (54, ConstantNode (IntVal 1 0), IntegerStamp 32 (- 2147483648) 2147483647),
-    (24, IfNode 53 23 22, VoidStamp),
-    (53, ConstantNode (IntVal 1 1), IntegerStamp 32 (- 2147483648) 2147483647),
-    (12, IfNode 52 11 10, VoidStamp),
-    (52, ConstantNode (IntVal 1 0), IntegerStamp 32 (- 2147483648) 2147483647),
-    (0, StartNode (Some 2) 7, VoidStamp),
-    (1, ParameterNode 0, IntegerStamp 32 (- 2147483648) 2147483647),
-    (2, FrameState [] None None None, IllegalStamp),
-    (3, ConstantNode (IntVal 32 0), IntegerStamp 32 0 0),
-    (4, IntegerEqualsNode 1 3, VoidStamp), (5, BeginNode 39, VoidStamp),
-    (6, BeginNode 12, VoidStamp), (7, IfNode 4 6 5, VoidStamp),
-    (8, ConstantNode (IntVal 32 5), IntegerStamp 32 5 5),
-    (9, IntegerEqualsNode 1 8, VoidStamp), (10, BeginNode 16, VoidStamp),
-    (11, BeginNode 14, VoidStamp), 
-    (12, IfNode 9 11 10, VoidStamp),
-    (13, ConstantNode (IntVal 32 100), IntegerStamp 32 100 100),
-    (14,
-     StoreFieldNode 14
-      ''org.graalvm.compiler.core.test.ConditionalEliminationTestBase::sink2'' 13
-      (Some 15) None 18,
-     VoidStamp),
-    (15, FrameState [] None None None, IllegalStamp), (16, EndNode, VoidStamp),
-    (17, MergeNode [16, 18] (Some 19) 24, VoidStamp), (18, EndNode, VoidStamp),
-    (19, FrameState [] None None None, IllegalStamp),
-    (20, ConstantNode (IntVal 32 101), IntegerStamp 32 101 101),
-    (21, IntegerLessThanNode 1 20, VoidStamp), (22, BeginNode 30, VoidStamp),
-    (23, BeginNode 25, VoidStamp), (24, IfNode 21 23 22, VoidStamp),
-    (25, EndNode, VoidStamp), (26, MergeNode [25, 27, 34] (Some 35) 43, VoidStamp),
-    (27, EndNode, VoidStamp), (28, BeginNode 32, VoidStamp),
-    (29, BeginNode 27, VoidStamp), (30, IfNode 4 28 29, VoidStamp),
-    (31, ConstantNode (IntVal 32 200), IntegerStamp 32 200 200),
-    (32,
-     StoreFieldNode 32
-      ''org.graalvm.compiler.core.test.ConditionalEliminationTest1::sink3'' 31
-      (Some 33) None 34,
-     VoidStamp),
-    (33, FrameState [] None None None, IllegalStamp), (34, EndNode, VoidStamp),
-    (35, FrameState [] None None None, IllegalStamp),
-    (36, ConstantNode (IntVal 32 2), IntegerStamp 32 2 2),
-    (37, IntegerEqualsNode 1 36, VoidStamp), (38, BeginNode 45, VoidStamp),
-    (39, EndNode, VoidStamp), (40, MergeNode [39, 41, 47] (Some 48) 49, VoidStamp),
-    (41, EndNode, VoidStamp), (42, BeginNode 41, VoidStamp),
-    (43, IfNode 37 42 38, VoidStamp),
-    (44, ConstantNode (IntVal 32 1), IntegerStamp 32 1 1),
-    (45,
-     StoreFieldNode 45
-      ''org.graalvm.compiler.core.test.ConditionalEliminationTestBase::sink1'' 44
-      (Some 46) None 47,
-     VoidStamp),
-    (46, FrameState [] None None None, IllegalStamp), (47, EndNode, VoidStamp),
-    (48, FrameState [] None None None, IllegalStamp),
-    (49,
-     StoreFieldNode 49
-      ''org.graalvm.compiler.core.test.ConditionalEliminationTestBase::sink0'' 3
-      (Some 50) None 51,
-     VoidStamp),
-    (50, FrameState [] None None None, IllegalStamp),
-    (51, ReturnNode None None, VoidStamp)]"
+value "
+  eqGraph
+  (Predicate.the
+    (ConditionalEliminationPhase_i_i_o
+      ConditionalEliminationTest1_test1Snippet_initial
+      (0, {}, ConditionalEliminationPhaseAnalysisStart)
+    ))
+  ConditionalEliminationTest1_test1Snippet_final
+"
 
-(* compare test1Snippet_basic, isabelle optimised graph vs graal optimised graph *)
-(* Works for now *)
-value "eqGraph ConditionalEliminationTest1_test1Snippet_isabelle ConditionalEliminationTest1_test1Snippet_final"
+value "
+  diffNodesGraph
+  (Predicate.the
+    (ConditionalEliminationPhase_i_i_o
+      ConditionalEliminationTest1_test1Snippet_initial
+      (0, {}, ConditionalEliminationPhaseAnalysisStart)
+    ))
+  ConditionalEliminationTest1_test1Snippet_final
+"
 
-
-
-
-
-
+value "
+  diffNodesInfo
+  (Predicate.the
+    (ConditionalEliminationPhase_i_i_o
+      ConditionalEliminationTest1_test1Snippet_initial
+      (0, {}, ConditionalEliminationPhaseAnalysisStart)
+    ))
+  ConditionalEliminationTest1_test1Snippet_final
+"
 
 
 (* initial: ConditionalEliminationTest1_test2Snippet*)
-definition ConditionalEliminationTest1_test2Snippet_initial :: IRGraph where
-  "ConditionalEliminationTest1_test2Snippet_initial = irgraph [
-  (0, (StartNode  (Some 2) 7), VoidStamp),
+definition ConditionalEliminationTest1_test2Snippet_initial :: IRGraph where  "ConditionalEliminationTest1_test2Snippet_initial = irgraph [
+  (0, (StartNode (Some 2) 7), VoidStamp),
   (1, (ParameterNode 0), IntegerStamp 32 (-2147483648) (2147483647)),
-  (2, (FrameState []  None None None), IllegalStamp),
+  (2, (FrameState [] None None None), IllegalStamp),
   (3, (ConstantNode (IntVal 32 (0))), IntegerStamp 32 (0) (0)),
   (4, (IntegerEqualsNode 1 3), VoidStamp),
   (5, (BeginNode 28), VoidStamp),
@@ -346,40 +1083,39 @@ definition ConditionalEliminationTest1_test2Snippet_initial :: IRGraph where
   (12, (BeginNode 14), VoidStamp),
   (13, (IfNode 10 12 11), VoidStamp),
   (14, (EndNode), VoidStamp),
-  (15, (MergeNode  [14, 16, 23]  (Some 24) 32), VoidStamp),
+  (15, (MergeNode  [14, 16, 23] (Some 24) 32), VoidStamp),
   (16, (EndNode), VoidStamp),
   (17, (BeginNode 21), VoidStamp),
   (18, (BeginNode 16), VoidStamp),
   (19, (IfNode 4 17 18), VoidStamp),
   (20, (ConstantNode (IntVal 32 (200))), IntegerStamp 32 (200) (200)),
-  (21, (StoreFieldNode 21 ''org.graalvm.compiler.core.test.ConditionalEliminationTest1::sink3'' 20  (Some 22)  None 23), VoidStamp),
-  (22, (FrameState []  None None None), IllegalStamp),
+  (21, (StoreFieldNode 21 ''org.graalvm.compiler.core.test.ConditionalEliminationTest1::sink3'' 20 (Some 22) None 23), VoidStamp),
+  (22, (FrameState [] None None None), IllegalStamp),
   (23, (EndNode), VoidStamp),
-  (24, (FrameState []  None None None), IllegalStamp),
+  (24, (FrameState [] None None None), IllegalStamp),
   (25, (ConstantNode (IntVal 32 (2))), IntegerStamp 32 (2) (2)),
   (26, (IntegerEqualsNode 1 25), VoidStamp),
   (27, (BeginNode 34), VoidStamp),
   (28, (EndNode), VoidStamp),
-  (29, (MergeNode  [28, 30, 36]  (Some 37) 38), VoidStamp),
+  (29, (MergeNode  [28, 30, 36] (Some 37) 38), VoidStamp),
   (30, (EndNode), VoidStamp),
   (31, (BeginNode 30), VoidStamp),
   (32, (IfNode 26 31 27), VoidStamp),
   (33, (ConstantNode (IntVal 32 (1))), IntegerStamp 32 (1) (1)),
-  (34, (StoreFieldNode 34 ''org.graalvm.compiler.core.test.ConditionalEliminationTestBase::sink1'' 33  (Some 35)  None 36), VoidStamp),
-  (35, (FrameState []  None None None), IllegalStamp),
+  (34, (StoreFieldNode 34 ''org.graalvm.compiler.core.test.ConditionalEliminationTestBase::sink1'' 33 (Some 35) None 36), VoidStamp),
+  (35, (FrameState [] None None None), IllegalStamp),
   (36, (EndNode), VoidStamp),
-  (37, (FrameState []  None None None), IllegalStamp),
-  (38, (StoreFieldNode 38 ''org.graalvm.compiler.core.test.ConditionalEliminationTestBase::sink0'' 3  (Some 39)  None 40), VoidStamp),
-  (39, (FrameState []  None None None), IllegalStamp),
-  (40, (ReturnNode  None  None), VoidStamp)
+  (37, (FrameState [] None None None), IllegalStamp),
+  (38, (StoreFieldNode 38 ''org.graalvm.compiler.core.test.ConditionalEliminationTestBase::sink0'' 3 (Some 39) None 40), VoidStamp),
+  (39, (FrameState [] None None None), IllegalStamp),
+  (40, (ReturnNode None None), VoidStamp)
   ]"
 
 (* final: ConditionalEliminationTest1_test2Snippet*)
-definition ConditionalEliminationTest1_test2Snippet_final :: IRGraph where
-  "ConditionalEliminationTest1_test2Snippet_final = irgraph [
-  (0, (StartNode  (Some 2) 7), VoidStamp),
+definition ConditionalEliminationTest1_test2Snippet_final :: IRGraph where  "ConditionalEliminationTest1_test2Snippet_final = irgraph [
+  (0, (StartNode (Some 2) 7), VoidStamp),
   (1, (ParameterNode 0), IntegerStamp 32 (-2147483648) (2147483647)),
-  (2, (FrameState []  None None None), IllegalStamp),
+  (2, (FrameState [] None None None), IllegalStamp),
   (3, (ConstantNode (IntVal 32 (0))), IntegerStamp 32 (0) (0)),
   (4, (IntegerEqualsNode 1 3), VoidStamp),
   (5, (BeginNode 28), VoidStamp),
@@ -392,100 +1128,72 @@ definition ConditionalEliminationTest1_test2Snippet_final :: IRGraph where
   (12, (BeginNode 14), VoidStamp),
   (13, (IfNode 41 12 11), VoidStamp),
   (14, (EndNode), VoidStamp),
-  (15, (MergeNode  [14, 16, 23]  (Some 24) 32), VoidStamp),
+  (15, (MergeNode  [14, 16, 23] (Some 24) 32), VoidStamp),
   (16, (EndNode), VoidStamp),
   (17, (BeginNode 21), VoidStamp),
   (18, (BeginNode 16), VoidStamp),
   (19, (IfNode 41 17 18), VoidStamp),
   (20, (ConstantNode (IntVal 32 (200))), IntegerStamp 32 (200) (200)),
-  (21, (StoreFieldNode 21 ''org.graalvm.compiler.core.test.ConditionalEliminationTest1::sink3'' 20  (Some 22)  None 23), VoidStamp),
-  (22, (FrameState []  None None None), IllegalStamp),
+  (21, (StoreFieldNode 21 ''org.graalvm.compiler.core.test.ConditionalEliminationTest1::sink3'' 20 (Some 22) None 23), VoidStamp),
+  (22, (FrameState [] None None None), IllegalStamp),
   (23, (EndNode), VoidStamp),
-  (24, (FrameState []  None None None), IllegalStamp),
+  (24, (FrameState [] None None None), IllegalStamp),
   (25, (ConstantNode (IntVal 32 (2))), IntegerStamp 32 (2) (2)),
   (26, (IntegerEqualsNode 1 25), VoidStamp),
   (27, (BeginNode 34), VoidStamp),
   (28, (EndNode), VoidStamp),
-  (29, (MergeNode  [28, 30, 36]  (Some 37) 38), VoidStamp),
+  (29, (MergeNode  [28, 30, 36] (Some 37) 38), VoidStamp),
   (30, (EndNode), VoidStamp),
   (31, (BeginNode 30), VoidStamp),
   (32, (IfNode 42 31 27), VoidStamp),
   (33, (ConstantNode (IntVal 32 (1))), IntegerStamp 32 (1) (1)),
-  (34, (StoreFieldNode 34 ''org.graalvm.compiler.core.test.ConditionalEliminationTestBase::sink1'' 33  (Some 35)  None 36), VoidStamp),
-  (35, (FrameState []  None None None), IllegalStamp),
+  (34, (StoreFieldNode 34 ''org.graalvm.compiler.core.test.ConditionalEliminationTestBase::sink1'' 33 (Some 35) None 36), VoidStamp),
+  (35, (FrameState [] None None None), IllegalStamp),
   (36, (EndNode), VoidStamp),
-  (37, (FrameState []  None None None), IllegalStamp),
-  (38, (StoreFieldNode 38 ''org.graalvm.compiler.core.test.ConditionalEliminationTestBase::sink0'' 3  (Some 39)  None 40), VoidStamp),
-  (39, (FrameState []  None None None), IllegalStamp),
-  (40, (ReturnNode  None  None), VoidStamp),
-  (41, (ConstantNode (IntVal 1 (1))), VoidStamp),
-  (42, (ConstantNode (IntVal 1 (0))), VoidStamp)
+  (37, (FrameState [] None None None), IllegalStamp),
+  (38, (StoreFieldNode 38 ''org.graalvm.compiler.core.test.ConditionalEliminationTestBase::sink0'' 3 (Some 39) None 40), VoidStamp),
+  (39, (FrameState [] None None None), IllegalStamp),
+  (40, (ReturnNode None None), VoidStamp),
+  (41, (LogicConstantNode (IntVal 1 (1))), VoidStamp),
+  (42, (LogicConstantNode (IntVal 1 (0))), VoidStamp)
   ]"
 
+value "
+  eqGraph
+  (Predicate.the
+    (ConditionalEliminationPhase_i_i_o
+      ConditionalEliminationTest1_test2Snippet_initial
+      (0, {}, ConditionalEliminationPhaseAnalysisStart)
+    ))
+  ConditionalEliminationTest1_test2Snippet_final
+"
 
-values "{g' . ConditionalEliminationPhase ConditionalEliminationTest1_test2Snippet_initial  (0, {}, [], []) g'}"
-definition ConditionalEliminationTest1_test2Snippet_isabelle :: IRGraph where
-  "ConditionalEliminationTest1_test2Snippet_isabelle = irgraph
-   [(32, IfNode 42 31 27, VoidStamp),
-    (42, ConstantNode (IntVal 1 0), IntegerStamp 32 (- 2147483648) 2147483647),
-    (13, IfNode 41 12 11, VoidStamp),
-    (41, ConstantNode (IntVal 1 1), IntegerStamp 32 (- 2147483648) 2147483647),
-    (0, StartNode (Some 2) 7, VoidStamp),
-    (1, ParameterNode 0, IntegerStamp 32 (- 2147483648) 2147483647),
-    (2, FrameState [] None None None, IllegalStamp),
-    (3, ConstantNode (IntVal 32 0), IntegerStamp 32 0 0),
-    (4, IntegerEqualsNode 1 3, VoidStamp), (5, BeginNode 28, VoidStamp),
-    (6, BeginNode 13, VoidStamp), (7, IfNode 4 6 5, VoidStamp),
-    (8, ConstantNode (IntVal 32 100), IntegerStamp 32 100 100),
-    (9, ConstantNode (IntVal 32 101), IntegerStamp 32 101 101),
-    (10, IntegerLessThanNode 1 9, VoidStamp), (11, BeginNode 19, VoidStamp),
-    (12, BeginNode 14, VoidStamp), (13, IfNode 10 12 11, VoidStamp),
-    (14, EndNode, VoidStamp), (15, MergeNode [14, 16, 23] (Some 24) 32, VoidStamp),
-    (16, EndNode, VoidStamp), (17, BeginNode 21, VoidStamp),
-    (18, BeginNode 16, VoidStamp), (19, IfNode 4 17 18, VoidStamp),
-    (20, ConstantNode (IntVal 32 200), IntegerStamp 32 200 200),
-    (21,
-     StoreFieldNode 21
-      ''org.graalvm.compiler.core.test.ConditionalEliminationTest1::sink3'' 20
-      (Some 22) None 23,
-     VoidStamp),
-    (22, FrameState [] None None None, IllegalStamp), (23, EndNode, VoidStamp),
-    (24, FrameState [] None None None, IllegalStamp),
-    (25, ConstantNode (IntVal 32 2), IntegerStamp 32 2 2),
-    (26, IntegerEqualsNode 1 25, VoidStamp), (27, BeginNode 34, VoidStamp),
-    (28, EndNode, VoidStamp), (29, MergeNode [28, 30, 36] (Some 37) 38, VoidStamp),
-    (30, EndNode, VoidStamp), (31, BeginNode 30, VoidStamp),
-    (32, IfNode 26 31 27, VoidStamp),
-    (33, ConstantNode (IntVal 32 1), IntegerStamp 32 1 1),
-    (34,
-     StoreFieldNode 34
-      ''org.graalvm.compiler.core.test.ConditionalEliminationTestBase::sink1'' 33
-      (Some 35) None 36,
-     VoidStamp),
-    (35, FrameState [] None None None, IllegalStamp), (36, EndNode, VoidStamp),
-    (37, FrameState [] None None None, IllegalStamp),
-    (38,
-     StoreFieldNode 38
-      ''org.graalvm.compiler.core.test.ConditionalEliminationTestBase::sink0'' 3
-      (Some 39) None 40,
-     VoidStamp),
-    (39, FrameState [] None None None, IllegalStamp),
-    (40, ReturnNode None None, VoidStamp)]"
+value "
+  diffNodesGraph
+  (Predicate.the
+    (ConditionalEliminationPhase_i_i_o
+      ConditionalEliminationTest1_test2Snippet_initial
+      (0, {}, ConditionalEliminationPhaseAnalysisStart)
+    ))
+  ConditionalEliminationTest1_test2Snippet_final
+"
 
-(* Graphs are not equal because current isabelle optimisation isn't flow sensitive/don't consider InfoElements *) 
-value "diffNodesGraph ConditionalEliminationTest1_test2Snippet_isabelle ConditionalEliminationTest1_test2Snippet_final"
-value "eqGraph ConditionalEliminationTest1_test2Snippet_isabelle ConditionalEliminationTest1_test2Snippet_final"
-
-
-
+value "
+  diffNodesInfo
+  (Predicate.the
+    (ConditionalEliminationPhase_i_i_o
+      ConditionalEliminationTest1_test2Snippet_initial
+      (0, {}, ConditionalEliminationPhaseAnalysisStart)
+    ))
+  ConditionalEliminationTest1_test2Snippet_final
+"
 
 
 (* initial: ConditionalEliminationTest1_test3Snippet*)
-definition ConditionalEliminationTest1_test3Snippet_initial :: IRGraph where
-  "ConditionalEliminationTest1_test3Snippet_initial = irgraph [
-  (0, (StartNode  (Some 2) 7), VoidStamp),
+definition ConditionalEliminationTest1_test3Snippet_initial :: IRGraph where  "ConditionalEliminationTest1_test3Snippet_initial = irgraph [
+  (0, (StartNode (Some 2) 7), VoidStamp),
   (1, (ParameterNode 0), IntegerStamp 32 (-2147483648) (2147483647)),
-  (2, (FrameState []  None None None), IllegalStamp),
+  (2, (FrameState [] None None None), IllegalStamp),
   (3, (ConstantNode (IntVal 32 (0))), IntegerStamp 32 (0) (0)),
   (4, (IntegerEqualsNode 1 3), VoidStamp),
   (5, (BeginNode 10), VoidStamp),
@@ -494,7 +1202,7 @@ definition ConditionalEliminationTest1_test3Snippet_initial :: IRGraph where
   (8, (ConstantNode (IntVal 32 (1))), IntegerStamp 32 (1) (1)),
   (9, (IntegerLessThanNode 1 8), VoidStamp),
   (10, (EndNode), VoidStamp),
-  (11, (MergeNode  [10, 12, 18, 24, 31, 37, 43, 53, 56]  (Some 57) 58), VoidStamp),
+  (11, (MergeNode  [10, 12, 18, 24, 31, 37, 43, 53, 56] (Some 57) 58), VoidStamp),
   (12, (EndNode), VoidStamp),
   (13, (BeginNode 21), VoidStamp),
   (14, (BeginNode 12), VoidStamp),
@@ -534,24 +1242,23 @@ definition ConditionalEliminationTest1_test3Snippet_initial :: IRGraph where
   (48, (BeginNode 51), VoidStamp),
   (49, (IfNode 46 48 47), VoidStamp),
   (50, (ConstantNode (IntVal 32 (42))), IntegerStamp 32 (42) (42)),
-  (51, (StoreFieldNode 51 ''org.graalvm.compiler.core.test.ConditionalEliminationTestBase::sink2'' 50  (Some 52)  None 53), VoidStamp),
-  (52, (FrameState []  None None None), IllegalStamp),
+  (51, (StoreFieldNode 51 ''org.graalvm.compiler.core.test.ConditionalEliminationTestBase::sink2'' 50 (Some 52) None 53), VoidStamp),
+  (52, (FrameState [] None None None), IllegalStamp),
   (53, (EndNode), VoidStamp),
-  (54, (StoreFieldNode 54 ''org.graalvm.compiler.core.test.ConditionalEliminationTestBase::sink1'' 8  (Some 55)  None 56), VoidStamp),
-  (55, (FrameState []  None None None), IllegalStamp),
+  (54, (StoreFieldNode 54 ''org.graalvm.compiler.core.test.ConditionalEliminationTestBase::sink1'' 8 (Some 55) None 56), VoidStamp),
+  (55, (FrameState [] None None None), IllegalStamp),
   (56, (EndNode), VoidStamp),
-  (57, (FrameState []  None None None), IllegalStamp),
-  (58, (StoreFieldNode 58 ''org.graalvm.compiler.core.test.ConditionalEliminationTestBase::sink0'' 3  (Some 59)  None 60), VoidStamp),
-  (59, (FrameState []  None None None), IllegalStamp),
-  (60, (ReturnNode  None  None), VoidStamp)
+  (57, (FrameState [] None None None), IllegalStamp),
+  (58, (StoreFieldNode 58 ''org.graalvm.compiler.core.test.ConditionalEliminationTestBase::sink0'' 3 (Some 59) None 60), VoidStamp),
+  (59, (FrameState [] None None None), IllegalStamp),
+  (60, (ReturnNode None None), VoidStamp)
   ]"
 
 (* final: ConditionalEliminationTest1_test3Snippet*)
-definition ConditionalEliminationTest1_test3Snippet_final :: IRGraph where
-  "ConditionalEliminationTest1_test3Snippet_final = irgraph [
-  (0, (StartNode  (Some 2) 7), VoidStamp),
+definition ConditionalEliminationTest1_test3Snippet_final :: IRGraph where  "ConditionalEliminationTest1_test3Snippet_final = irgraph [
+  (0, (StartNode (Some 2) 7), VoidStamp),
   (1, (ParameterNode 0), IntegerStamp 32 (-2147483648) (2147483647)),
-  (2, (FrameState []  None None None), IllegalStamp),
+  (2, (FrameState [] None None None), IllegalStamp),
   (3, (ConstantNode (IntVal 32 (0))), IntegerStamp 32 (0) (0)),
   (4, (IntegerEqualsNode 1 3), VoidStamp),
   (5, (BeginNode 10), VoidStamp),
@@ -560,7 +1267,7 @@ definition ConditionalEliminationTest1_test3Snippet_final :: IRGraph where
   (8, (ConstantNode (IntVal 32 (1))), IntegerStamp 32 (1) (1)),
   (9, (IntegerLessThanNode 1 8), VoidStamp),
   (10, (EndNode), VoidStamp),
-  (11, (MergeNode  [10, 12, 18, 24, 31, 37, 43, 53, 56]  (Some 57) 58), VoidStamp),
+  (11, (MergeNode  [10, 12, 18, 24, 31, 37, 43, 53, 56] (Some 57) 58), VoidStamp),
   (12, (EndNode), VoidStamp),
   (13, (BeginNode 21), VoidStamp),
   (14, (BeginNode 12), VoidStamp),
@@ -600,245 +1307,204 @@ definition ConditionalEliminationTest1_test3Snippet_final :: IRGraph where
   (48, (BeginNode 51), VoidStamp),
   (49, (IfNode 62 48 47), VoidStamp),
   (50, (ConstantNode (IntVal 32 (42))), IntegerStamp 32 (42) (42)),
-  (51, (StoreFieldNode 51 ''org.graalvm.compiler.core.test.ConditionalEliminationTestBase::sink2'' 50  (Some 52)  None 53), VoidStamp),
-  (52, (FrameState []  None None None), IllegalStamp),
+  (51, (StoreFieldNode 51 ''org.graalvm.compiler.core.test.ConditionalEliminationTestBase::sink2'' 50 (Some 52) None 53), VoidStamp),
+  (52, (FrameState [] None None None), IllegalStamp),
   (53, (EndNode), VoidStamp),
-  (54, (StoreFieldNode 54 ''org.graalvm.compiler.core.test.ConditionalEliminationTestBase::sink1'' 8  (Some 55)  None 56), VoidStamp),
-  (55, (FrameState []  None None None), IllegalStamp),
+  (54, (StoreFieldNode 54 ''org.graalvm.compiler.core.test.ConditionalEliminationTestBase::sink1'' 8 (Some 55) None 56), VoidStamp),
+  (55, (FrameState [] None None None), IllegalStamp),
   (56, (EndNode), VoidStamp),
-  (57, (FrameState []  None None None), IllegalStamp),
-  (58, (StoreFieldNode 58 ''org.graalvm.compiler.core.test.ConditionalEliminationTestBase::sink0'' 3  (Some 59)  None 60), VoidStamp),
-  (59, (FrameState []  None None None), IllegalStamp),
-  (60, (ReturnNode  None  None), VoidStamp),
-  (61, (ConstantNode (IntVal 1 (1))), VoidStamp),
-  (62, (ConstantNode (IntVal 1 (0))), VoidStamp)
+  (57, (FrameState [] None None None), IllegalStamp),
+  (58, (StoreFieldNode 58 ''org.graalvm.compiler.core.test.ConditionalEliminationTestBase::sink0'' 3 (Some 59) None 60), VoidStamp),
+  (59, (FrameState [] None None None), IllegalStamp),
+  (60, (ReturnNode None None), VoidStamp),
+  (61, (LogicConstantNode (IntVal 1 (1))), VoidStamp),
+  (62, (LogicConstantNode (IntVal 1 (0))), VoidStamp)
   ]"
 
-values "{g' . ConditionalEliminationPhase ConditionalEliminationTest1_test3Snippet_initial  (0, {}, [], []) g'}"
-definition ConditionalEliminationTest1_test3Snippet_isabelle :: IRGraph where
-  "ConditionalEliminationTest1_test3Snippet_isabelle  = irgraph [
-    (33, IfNode 64 32 30, VoidStamp),
-    (64, ConstantNode (IntVal 1 0), IntegerStamp 32 (- 2147483648) 2147483647),
-    (27, IfNode 63 25 26, VoidStamp),
-    (63, ConstantNode (IntVal 1 1), IntegerStamp 32 (- 2147483648) 2147483647),
-    (21, IfNode 62 19 20, VoidStamp),
-    (62, ConstantNode (IntVal 1 1), IntegerStamp 32 (- 2147483648) 2147483647),
-    (15, IfNode 61 13 14, VoidStamp),
-    (61, ConstantNode (IntVal 1 1), IntegerStamp 32 (- 2147483648) 2147483647),
-    (0, StartNode (Some 2) 7, VoidStamp),
-    (1, ParameterNode 0, IntegerStamp 32 (- 2147483648) 2147483647),
-    (2, FrameState [] None None None, IllegalStamp),
-    (3, ConstantNode (IntVal 32 0), IntegerStamp 32 0 0),
-    (4, IntegerEqualsNode 1 3, VoidStamp), (5, BeginNode 10, VoidStamp),
-    (6, BeginNode 15, VoidStamp), (7, IfNode 4 6 5, VoidStamp),
-    (8, ConstantNode (IntVal 32 1), IntegerStamp 32 1 1),
-    (9, IntegerLessThanNode 1 8, VoidStamp), (10, EndNode, VoidStamp),
-    (11, MergeNode [10, 12, 18, 24, 31, 37, 43, 53, 56] (Some 57) 58, VoidStamp),
-    (12, EndNode, VoidStamp), (13, BeginNode 21, VoidStamp),
-    (14, BeginNode 12, VoidStamp), (15, IfNode 9 13 14, VoidStamp),
-    (16, ConstantNode (IntVal 32 2), IntegerStamp 32 2 2),
-    (17, IntegerLessThanNode 1 16, VoidStamp), (18, EndNode, VoidStamp),
-    (19, BeginNode 27, VoidStamp), (20, BeginNode 18, VoidStamp),
-    (21, IfNode 17 19 20, VoidStamp),
-    (22, ConstantNode (IntVal 32 3), IntegerStamp 32 3 3),
-    (23, IntegerLessThanNode 1 22, VoidStamp), (24, EndNode, VoidStamp),
-    (25, BeginNode 33, VoidStamp), (26, BeginNode 24, VoidStamp),
-    (27, IfNode 23 25 26, VoidStamp),
-    (28, ConstantNode (IntVal 32 (- 1)), IntegerStamp 32 (- 1) (- 1)),
-    (29, IntegerLessThanNode 1 3, VoidStamp), (30, BeginNode 39, VoidStamp),
-    (31, EndNode, VoidStamp), (32, BeginNode 31, VoidStamp),
-    (33, IfNode 29 32 30, VoidStamp),
-    (34, ConstantNode (IntVal 32 (- 2)), IntegerStamp 32 (- 2) (- 2)),
-    (35, IntegerLessThanNode 1 28, VoidStamp), (36, BeginNode 45, VoidStamp),
-    (37, EndNode, VoidStamp), (38, BeginNode 37, VoidStamp),
-    (39, IfNode 35 38 36, VoidStamp),
-    (40, ConstantNode (IntVal 32 (- 3)), IntegerStamp 32 (- 3) (- 3)),
-    (41, IntegerLessThanNode 1 34, VoidStamp), (42, BeginNode 49, VoidStamp),
-    (43, EndNode, VoidStamp), (44, BeginNode 43, VoidStamp),
-    (45, IfNode 41 44 42, VoidStamp), (46, IntegerEqualsNode 1 8, VoidStamp),
-    (47, BeginNode 54, VoidStamp), (48, BeginNode 51, VoidStamp),
-    (49, IfNode 46 48 47, VoidStamp),
-    (50, ConstantNode (IntVal 32 42), IntegerStamp 32 42 42),
-    (51,
-     StoreFieldNode 51
-      ''org.graalvm.compiler.core.test.ConditionalEliminationTestBase::sink2'' 50
-      (Some 52) None 53,
-     VoidStamp),
-    (52, FrameState [] None None None, IllegalStamp), (53, EndNode, VoidStamp),
-    (54,
-     StoreFieldNode 54
-      ''org.graalvm.compiler.core.test.ConditionalEliminationTestBase::sink1'' 8
-      (Some 55) None 56,
-     VoidStamp),
-    (55, FrameState [] None None None, IllegalStamp), (56, EndNode, VoidStamp),
-    (57, FrameState [] None None None, IllegalStamp),
-    (58,
-     StoreFieldNode 58
-      ''org.graalvm.compiler.core.test.ConditionalEliminationTestBase::sink0'' 3
-      (Some 59) None 60,
-     VoidStamp),
-    (59, FrameState [] None None None, IllegalStamp),
-    (60, ReturnNode None None, VoidStamp)]"
+value "
+  eqGraph
+  (Predicate.the
+    (ConditionalEliminationPhase_i_i_o
+      ConditionalEliminationTest1_test3Snippet_initial
+      (0, {}, ConditionalEliminationPhaseAnalysisStart)
+    ))
+  ConditionalEliminationTest1_test3Snippet_final
+"
 
-(* Fails. Optimisation for this node in Graal uses tryFold and flow typing *)
-value "diffNodesGraph ConditionalEliminationTest1_test3Snippet_isabelle ConditionalEliminationTest1_test3Snippet_final"
-value "eqGraph ConditionalEliminationTest1_test3Snippet_isabelle ConditionalEliminationTest1_test3Snippet_final"
+value "
+  diffNodesGraph
+  (Predicate.the
+    (ConditionalEliminationPhase_i_i_o
+      ConditionalEliminationTest1_test3Snippet_initial
+      (0, {}, ConditionalEliminationPhaseAnalysisStart)
+    ))
+  ConditionalEliminationTest1_test3Snippet_final
+"
 
-
-
-
-
+value "
+  diffNodesInfo
+  (Predicate.the
+    (ConditionalEliminationPhase_i_i_o
+      ConditionalEliminationTest1_test3Snippet_initial
+      (0, {}, ConditionalEliminationPhaseAnalysisStart)
+    ))
+  ConditionalEliminationTest1_test3Snippet_final
+"
 
 
 (* initial: ConditionalEliminationTest4_test1Snippet*)
-definition ConditionalEliminationTest4_test1Snippet_initial :: IRGraph where
-  "ConditionalEliminationTest4_test1Snippet_initial = irgraph [
-  (0, (StartNode  (Some 3) 7), VoidStamp),
+definition ConditionalEliminationTest4_test1Snippet_initial :: IRGraph where  "ConditionalEliminationTest4_test1Snippet_initial = irgraph [
+  (0, (StartNode (Some 3) 7), VoidStamp),
   (1, (ParameterNode 0), IntegerStamp 32 (-2147483648) (2147483647)),
   (2, (ParameterNode 1), IntegerStamp 32 (-2147483648) (2147483647)),
-  (3, (FrameState []  None None None), IllegalStamp),
+  (3, (FrameState [] None None None), IllegalStamp),
   (4, (IntegerLessThanNode 2 1), VoidStamp),
   (5, (BeginNode 8), VoidStamp),
   (6, (BeginNode 13), VoidStamp),
   (7, (IfNode 4 6 5), VoidStamp),
   (8, (EndNode), VoidStamp),
-  (9, (MergeNode  [8, 10]  (Some 16) 18), VoidStamp),
+  (9, (MergeNode  [8, 10] (Some 16) 18), VoidStamp),
   (10, (EndNode), VoidStamp),
   (11, (BeginNode 15), VoidStamp),
   (12, (BeginNode 10), VoidStamp),
   (13, (IfNode 4 11 12), VoidStamp),
   (14, (ConstantNode (IntVal 32 (1))), IntegerStamp 32 (1) (1)),
-  (15, (ReturnNode  (Some 14)  None), VoidStamp),
-  (16, (FrameState []  None None None), IllegalStamp),
+  (15, (ReturnNode (Some 14) None), VoidStamp),
+  (16, (FrameState [] None None None), IllegalStamp),
   (17, (ConstantNode (IntVal 32 (2))), IntegerStamp 32 (2) (2)),
-  (18, (ReturnNode  (Some 17)  None), VoidStamp)
+  (18, (ReturnNode (Some 17) None), VoidStamp)
   ]"
 
 (* final: ConditionalEliminationTest4_test1Snippet*)
-definition ConditionalEliminationTest4_test1Snippet_final :: IRGraph where
-  "ConditionalEliminationTest4_test1Snippet_final = irgraph [
-  (0, (StartNode  (Some 3) 7), VoidStamp),
+definition ConditionalEliminationTest4_test1Snippet_final :: IRGraph where  "ConditionalEliminationTest4_test1Snippet_final = irgraph [
+  (0, (StartNode (Some 3) 7), VoidStamp),
   (1, (ParameterNode 0), IntegerStamp 32 (-2147483648) (2147483647)),
   (2, (ParameterNode 1), IntegerStamp 32 (-2147483648) (2147483647)),
-  (3, (FrameState []  None None None), IllegalStamp),
+  (3, (FrameState [] None None None), IllegalStamp),
   (4, (IntegerLessThanNode 2 1), VoidStamp),
   (5, (BeginNode 8), VoidStamp),
   (6, (BeginNode 13), VoidStamp),
   (7, (IfNode 4 6 5), VoidStamp),
   (8, (EndNode), VoidStamp),
-  (9, (MergeNode  [8, 10]  (Some 16) 18), VoidStamp),
+  (9, (MergeNode  [8, 10] (Some 16) 18), VoidStamp),
   (10, (EndNode), VoidStamp),
   (11, (BeginNode 15), VoidStamp),
   (12, (BeginNode 10), VoidStamp),
   (13, (IfNode 19 11 12), VoidStamp),
   (14, (ConstantNode (IntVal 32 (1))), IntegerStamp 32 (1) (1)),
-  (15, (ReturnNode  (Some 14)  None), VoidStamp),
-  (16, (FrameState []  None None None), IllegalStamp),
+  (15, (ReturnNode (Some 14) None), VoidStamp),
+  (16, (FrameState [] None None None), IllegalStamp),
   (17, (ConstantNode (IntVal 32 (2))), IntegerStamp 32 (2) (2)),
-  (18, (ReturnNode  (Some 17)  None), VoidStamp),
-  (19, (ConstantNode (IntVal 1 (1))), VoidStamp)
+  (18, (ReturnNode (Some 17) None), VoidStamp),
+  (19, (LogicConstantNode (IntVal 1 (1))), VoidStamp)
   ]"
 
-values "{g' . ConditionalEliminationPhase ConditionalEliminationTest4_test1Snippet_initial  (0, {}, [], []) g'}"
-definition ConditionalEliminationTest4_test1Snippet_isabelle :: IRGraph where
-  "ConditionalEliminationTest4_test1Snippet_isabelle = irgraph
-   [(13, IfNode 19 11 12, VoidStamp),
-    (19, ConstantNode (IntVal 1 1), IntegerStamp 32 (- 2147483648) 2147483647),
-    (0, StartNode (Some 3) 7, VoidStamp),
-    (1, ParameterNode 0, IntegerStamp 32 (- 2147483648) 2147483647),
-    (2, ParameterNode 1, IntegerStamp 32 (- 2147483648) 2147483647),
-    (3, FrameState [] None None None, IllegalStamp),
-    (4, IntegerLessThanNode 2 1, VoidStamp), (5, BeginNode 8, VoidStamp),
-    (6, BeginNode 13, VoidStamp), (7, IfNode 4 6 5, VoidStamp),
-    (8, EndNode, VoidStamp), (9, MergeNode [8, 10] (Some 16) 18, VoidStamp),
-    (10, EndNode, VoidStamp), (11, BeginNode 15, VoidStamp),
-    (12, BeginNode 10, VoidStamp), (13, IfNode 4 11 12, VoidStamp),
-    (14, ConstantNode (IntVal 32 1), IntegerStamp 32 1 1),
-    (15, ReturnNode (Some 14) None, VoidStamp),
-    (16, FrameState [] None None None, IllegalStamp),
-    (17, ConstantNode (IntVal 32 2), IntegerStamp 32 2 2),
-    (18, ReturnNode (Some 17) None, VoidStamp)]"
+value "
+  eqGraph
+  (Predicate.the
+    (ConditionalEliminationPhase_i_i_o
+      ConditionalEliminationTest4_test1Snippet_initial
+      (0, {}, ConditionalEliminationPhaseAnalysisStart)
+    ))
+  ConditionalEliminationTest4_test1Snippet_final
+"
 
-(* Works for now *)
-value "diffNodesGraph ConditionalEliminationTest4_test1Snippet_isabelle ConditionalEliminationTest4_test1Snippet_final"
-value "eqGraph ConditionalEliminationTest4_test1Snippet_isabelle ConditionalEliminationTest4_test1Snippet_final"
+value "
+  diffNodesGraph
+  (Predicate.the
+    (ConditionalEliminationPhase_i_i_o
+      ConditionalEliminationTest4_test1Snippet_initial
+      (0, {}, ConditionalEliminationPhaseAnalysisStart)
+    ))
+  ConditionalEliminationTest4_test1Snippet_final
+"
 
-
-
-
+value "
+  diffNodesInfo
+  (Predicate.the
+    (ConditionalEliminationPhase_i_i_o
+      ConditionalEliminationTest4_test1Snippet_initial
+      (0, {}, ConditionalEliminationPhaseAnalysisStart)
+    ))
+  ConditionalEliminationTest4_test1Snippet_final
+"
 
 
 (* initial: ConditionalEliminationTest4_test2Snippet*)
-definition ConditionalEliminationTest4_test2Snippet_initial :: IRGraph where
-  "ConditionalEliminationTest4_test2Snippet_initial = irgraph [
-  (0, (StartNode  (Some 3) 7), VoidStamp),
+definition ConditionalEliminationTest4_test2Snippet_initial :: IRGraph where  "ConditionalEliminationTest4_test2Snippet_initial = irgraph [
+  (0, (StartNode (Some 3) 7), VoidStamp),
   (1, (ParameterNode 0), IntegerStamp 32 (-2147483648) (2147483647)),
   (2, (ParameterNode 1), IntegerStamp 32 (-2147483648) (2147483647)),
-  (3, (FrameState []  None None None), IllegalStamp),
+  (3, (FrameState [] None None None), IllegalStamp),
   (4, (IntegerLessThanNode 1 2), VoidStamp),
   (5, (BeginNode 8), VoidStamp),
   (6, (BeginNode 13), VoidStamp),
   (7, (IfNode 4 6 5), VoidStamp),
   (8, (EndNode), VoidStamp),
-  (9, (MergeNode  [8, 10]  (Some 16) 18), VoidStamp),
+  (9, (MergeNode  [8, 10] (Some 16) 18), VoidStamp),
   (10, (EndNode), VoidStamp),
   (11, (BeginNode 15), VoidStamp),
   (12, (BeginNode 10), VoidStamp),
   (13, (IfNode 4 11 12), VoidStamp),
   (14, (ConstantNode (IntVal 32 (1))), IntegerStamp 32 (1) (1)),
-  (15, (ReturnNode  (Some 14)  None), VoidStamp),
-  (16, (FrameState []  None None None), IllegalStamp),
+  (15, (ReturnNode (Some 14) None), VoidStamp),
+  (16, (FrameState [] None None None), IllegalStamp),
   (17, (ConstantNode (IntVal 32 (2))), IntegerStamp 32 (2) (2)),
-  (18, (ReturnNode  (Some 17)  None), VoidStamp)
+  (18, (ReturnNode (Some 17) None), VoidStamp)
   ]"
 
 (* final: ConditionalEliminationTest4_test2Snippet*)
-definition ConditionalEliminationTest4_test2Snippet_final :: IRGraph where
-  "ConditionalEliminationTest4_test2Snippet_final = irgraph [
-  (0, (StartNode  (Some 3) 7), VoidStamp),
+definition ConditionalEliminationTest4_test2Snippet_final :: IRGraph where  "ConditionalEliminationTest4_test2Snippet_final = irgraph [
+  (0, (StartNode (Some 3) 7), VoidStamp),
   (1, (ParameterNode 0), IntegerStamp 32 (-2147483648) (2147483647)),
   (2, (ParameterNode 1), IntegerStamp 32 (-2147483648) (2147483647)),
-  (3, (FrameState []  None None None), IllegalStamp),
+  (3, (FrameState [] None None None), IllegalStamp),
   (4, (IntegerLessThanNode 1 2), VoidStamp),
   (5, (BeginNode 8), VoidStamp),
   (6, (BeginNode 13), VoidStamp),
   (7, (IfNode 4 6 5), VoidStamp),
   (8, (EndNode), VoidStamp),
-  (9, (MergeNode  [8, 10]  (Some 16) 18), VoidStamp),
+  (9, (MergeNode  [8, 10] (Some 16) 18), VoidStamp),
   (10, (EndNode), VoidStamp),
   (11, (BeginNode 15), VoidStamp),
   (12, (BeginNode 10), VoidStamp),
   (13, (IfNode 19 11 12), VoidStamp),
   (14, (ConstantNode (IntVal 32 (1))), IntegerStamp 32 (1) (1)),
-  (15, (ReturnNode  (Some 14)  None), VoidStamp),
-  (16, (FrameState []  None None None), IllegalStamp),
+  (15, (ReturnNode (Some 14) None), VoidStamp),
+  (16, (FrameState [] None None None), IllegalStamp),
   (17, (ConstantNode (IntVal 32 (2))), IntegerStamp 32 (2) (2)),
-  (18, (ReturnNode  (Some 17)  None), VoidStamp),
-  (19, (ConstantNode (IntVal 1 (1))), VoidStamp)
+  (18, (ReturnNode (Some 17) None), VoidStamp),
+  (19, (LogicConstantNode (IntVal 1 (1))), VoidStamp)
   ]"
 
-values "{g' . ConditionalEliminationPhase ConditionalEliminationTest4_test2Snippet_initial  (0, {}, [], []) g'}"
-definition ConditionalEliminationTest4_test2Snippet_isabelle :: IRGraph where
-  "ConditionalEliminationTest4_test2Snippet_isabelle = irgraph
-   [(13, IfNode 19 11 12, VoidStamp),
-    (19, ConstantNode (IntVal 1 1), IntegerStamp 32 (- 2147483648) 2147483647),
-    (0, StartNode (Some 3) 7, VoidStamp),
-    (1, ParameterNode 0, IntegerStamp 32 (- 2147483648) 2147483647),
-    (2, ParameterNode 1, IntegerStamp 32 (- 2147483648) 2147483647),
-    (3, FrameState [] None None None, IllegalStamp),
-    (4, IntegerLessThanNode 1 2, VoidStamp), (5, BeginNode 8, VoidStamp),
-    (6, BeginNode 13, VoidStamp), (7, IfNode 4 6 5, VoidStamp),
-    (8, EndNode, VoidStamp), (9, MergeNode [8, 10] (Some 16) 18, VoidStamp),
-    (10, EndNode, VoidStamp), (11, BeginNode 15, VoidStamp),
-    (12, BeginNode 10, VoidStamp), (13, IfNode 4 11 12, VoidStamp),
-    (14, ConstantNode (IntVal 32 1), IntegerStamp 32 1 1),
-    (15, ReturnNode (Some 14) None, VoidStamp),
-    (16, FrameState [] None None None, IllegalStamp),
-    (17, ConstantNode (IntVal 32 2), IntegerStamp 32 2 2),
-    (18, ReturnNode (Some 17) None, VoidStamp)]"
+value "
+  eqGraph
+  (Predicate.the
+    (ConditionalEliminationPhase_i_i_o
+      ConditionalEliminationTest4_test2Snippet_initial
+      (0, {}, ConditionalEliminationPhaseAnalysisStart)
+    ))
+  ConditionalEliminationTest4_test2Snippet_final
+"
 
-(* Works for now *)
-value "diffNodesGraph ConditionalEliminationTest4_test2Snippet_isabelle ConditionalEliminationTest4_test2Snippet_final"
-value "eqGraph ConditionalEliminationTest4_test2Snippet_isabelle ConditionalEliminationTest4_test2Snippet_final"
+value "
+  diffNodesGraph
+  (Predicate.the
+    (ConditionalEliminationPhase_i_i_o
+      ConditionalEliminationTest4_test2Snippet_initial
+      (0, {}, ConditionalEliminationPhaseAnalysisStart)
+    ))
+  ConditionalEliminationTest4_test2Snippet_final
+"
+
+value "
+  diffNodesInfo
+  (Predicate.the
+    (ConditionalEliminationPhase_i_i_o
+      ConditionalEliminationTest4_test2Snippet_initial
+      (0, {}, ConditionalEliminationPhaseAnalysisStart)
+    ))
+  ConditionalEliminationTest4_test2Snippet_final
+"
 
 end
